2013/7/17日版に差し替え 既存より新しい部分は未訳

Imp_J.v
@@ -1,77 +1,69 @@
-(** * Imp_J: 単純な命令型プログラム *)
+(** * Imp: Simple Imperative Programs *)
 
-(* $Date: 2011-06-22 14:56:13 -0400 (Wed, 22 Jun 2011) $ *)
+(* In this chapter, we begin a new direction that will continue for
+    the rest of the course.  Up to now most of our attention has been
+    focused on various aspects of Coq itself, while from now on we'll
+    mostly be using Coq to formalize other things.  (We'll continue to
+    pause from time to time to introduce a few additional aspects of
+    Coq.)
 
-(* In this chapter, we begin a new direction that we'll
-    continue for the rest of the course: up to now we've been mostly
-    studying Coq itself, but from now on we'll mostly be using Coq to
-    formalize other things.
-    
-    ...
-    This chapter looks at how to define the _syntax_ and _semantics_
-    of Imp; the chapters that follow develop a theory of _program
-    equivalence_ and introduce _Hoare Logic_, the best known logic for
-    reasoning about imperative programs. *)
+    Our first case study is a _simple imperative programming language_
+    called Imp, embodying a tiny core fragment of conventional
+    mainstream languages such as C and Java.  Here is a familiar
+    mathematical function written in Imp.
+*)
 (** この章では、コースの残りに続く新しい方向へ進み始めます。
     ここまではもっぱらCoq自身について学習してきましたが、ここからは、
-    主として別のものを形式化するためにCoqを使います。
+    主として別のものを形式化するためにCoqを使います。(ときどき、
+	いくつかのCoqの付加的な側面について紹介します)
     
     はじめの例は、Imp と呼ばれる単純な命令型プログラミング言語です。
+	CやJavaのような標準的な言語のコアな部分を抜き出したようなものです。
     下の例は、おなじみの数学的関数を Imp で書いたものです。
-[[
-     Z ::= X;
-     Y ::= 1;
+     Z ::= X;;
+     Y ::= 1;;
      WHILE not (Z = 0) DO
-       Y ::= Y * Z;
+       Y ::= Y * Z;;
        Z ::= Z - 1
      END
-]]
-    この章ではImpの構文(_syntax_)と意味(_semantics_)をどのように定義するかを見ます。
+*)
+
+(* This chapter looks at how to define the _syntax_ and _semantics_
+    of Imp; the chapters that follow develop a theory of _program
+    equivalence_ and introduce _Hoare Logic_, a widely used logic for
+    reasoning about imperative programs. *)
+(** この章ではImpの構文(_syntax_)と意味(_semantics_)をどのように定義するかを見ます。
     続く章では、プログラムの同値性(_program equivalence_)の理論を展開し、
     命令型プログラムについての推論のための論理として一番知られているホーア論理
     (_Hoare Logic_)を紹介します。 *)
 
 (* ####################################################### *)
-(* *** Sflib *)
 (** *** Sflib *)
 
-(* A minor technical point: Instead of asking Coq to import our
-    earlier definitions from [Logic.v], we import a small library
+(** A minor technical point: Instead of asking Coq to import our
+    earlier definitions from chapter [Logic], we import a small library
     called [Sflib.v], containing just a few definitions and theorems
     from earlier chapters that we'll actually use in the rest of the
-    course.  You won't notice much difference, since most of what's
+    course.  This change should be nearly invisible, since most of what's
     missing from Sflib has identical definitions in the Coq standard
-    library.  The main reason for doing this is to tidy the global Coq
+    library.  The main reason for doing it is to tidy the global Coq
     environment so that, for example, it is easier to search for
     relevant theorems. *)
-(** マイナーな技術的ポイント: ここまでの定義を[Logic_J.v]からインポートする代わりに、
-    [Sflib_J.v]という小さなライブラリをインポートします。
-    このライブラリは、前の章の定義や定理のうち、残りの章で実際に使うものだけを集めたものです。
-    読者はそれほど違うものとは感じないでしょう。というのは、
-    Sflib で抜けているもののほとんどは、Coqの標準ライブラリの定義と同じものだからです。
-    こうする主な理由は、Coqのグローバルな環境を整理して、例えば、
-    関係する定理を探すのを容易にするためです。 *)
 
-Require Export SfLib_J.
+Require Export SfLib.
 
 (* ####################################################### *)
-(* * Arithmetic and Boolean Expressions *)
-(** * 算術式とブール式 *)
+(** * Arithmetic and Boolean Expressions *)
 
-(* We'll present Imp in three parts: first a core language of
+(** We'll present Imp in three parts: first a core language of
     _arithmetic and boolean expressions_, then an extension of these
     expressions with _variables_, and finally a language of _commands_
     including assignment, conditions, sequencing, and loops. *)
-(** Impを三つの部分に分けて示します: 最初に算術式(_arithmetic expressions_)
-    とブール式(_boolean expressions_)、次にこれらの式に変数(_variables_)を加えたもの、
-    そして最後に代入(assignment)、条件分岐(conditions)、コマンド合成(sequencing)、
-    ループ(loops)を持つコマンド(_commands_)の言語です。*)
-
-Module AExp.
 
 (* ####################################################### *)
-(* ** Syntax *)
-(** ** 構文 *)
+(** ** Syntax *)
+
+Module AExp.
 
 (* These two definitions specify the _abstract syntax_ of
     arithmetic and boolean expressions. *)
@@ -95,12 +87,12 @@ Inductive bexp : Type :=
     concrete syntax that a programmer would actually write to these
     abstract syntax trees -- the process that, for example, would
     translate the string ["1+2*3"] to the AST [APlus (ANum
-    1) (AMult (ANum 2) (ANum 3))].  The file [ImpParser.v] develops a
-    simple implementation of a lexical analyzer and parser that can
-    perform this translation.  You do _not_ need to understand that
-    file to understand this one, but if you haven't taken a course
-    where these techniques are covered (e.g., a compilers course) you
-    may want to skim it. *)
+    1) (AMult (ANum 2) (ANum 3))].  The optional chapter [ImpParser]
+    develops a simple implementation of a lexical analyzer and parser
+    that can perform this translation.  You do _not_ need to
+    understand that file to understand this one, but if you haven't
+    taken a course where these techniques are covered (e.g., a
+    compilers course) you may want to skim it. *)
 (** この章では、プログラマが実際に書く具象構文から抽象構文木への変換は省略します。
     例えば、文字列["1+2*3"]をAST(Abstract Syntax Tree, 抽象構文木) 
     [APlus (ANum 1) (AMult (ANum 2) (ANum 3))] にする変換のことです。
@@ -109,37 +101,21 @@ Inductive bexp : Type :=
     もしそれらの技術についてのコース(例えばコンパイラコース)を受講していないならば、
     ざっと見てみるのも良いでしょう。 *)
 
-(* For comparison, here's a conventional BNF (Backus-Naur Form)
-    grammar defining the same abstract syntax:
-[[
-    aexp ::= nat
-           | aexp '+' aexp
-           | aexp '-' aexp
-           | aexp '*' aexp
-
-    bexp ::= true
-           | false
-           | aexp '=' aexp
-           | aexp '<=' aexp
-           | bexp 'and' bexp
-           | 'not' bexp
-]]
-*)
+(** For comparison, here's a conventional BNF (Backus-Naur Form)
+    grammar defining the same abstract syntax:*)
 (** 比較のため、同じ抽象構文を定義する慣習的なBNF(Backus-Naur Form)
     文法を以下に示します:
-[[
-    aexp ::= nat
-           | aexp '+' aexp
-           | aexp '-' aexp
-           | aexp '*' aexp
+    a ::= nat
+        | a + a
+        | a - a
+        | a * a
 
-    bexp ::= true
-           | false
-           | aexp '=' aexp
-           | aexp '<=' aexp
-           | bexp 'and' bexp
-           | 'not' bexp
-]]
+    b ::= true
+        | false
+        | a = a
+        | a <= a
+        | b and b
+        | not b
 *)
 
 (* Compared to the Coq version above...
@@ -157,14 +133,14 @@ Inductive bexp : Type :=
          The Coq version consistently omits all this information and
          concentrates on the abstract syntax only.
 
-       - On the other hand, the BNF version is lighter and arguably
+       - On the other hand, the BNF version is lighter and
          easier to read.  Its informality makes it flexible, which is
          a huge advantage in situations like discussions at the
          blackboard, where conveying general ideas is more important
          than getting every detail nailed down precisely.
 
          Indeed, there are dozens of BNF-like notations and people
-         switch freely among them, usually without bothering to which
+         switch freely among them, usually without bothering to say which
          form of BNF they're using because there is no need to: a
          rough-and-ready informal understanding is all that's
          needed. *)
@@ -190,23 +166,22 @@ Inductive bexp : Type :=
          通常はそれらのうちのどのBNFを使っているかを気にしません。
          その必要がないからです。おおざっぱな非形式的な理解だけが必要なのです。 *)
 
-(* It's good to be comfortable with both sorts of notations: informal
-    ones for communicating between humans and formal ones for carrying
-    out implementations and proofs. *)
+
+(* It's good to be comfortable with both sorts of notations:
+    informal ones for communicating between humans and formal ones for
+    carrying out implementations and proofs. *)
 (** 両方の記法に通じているのは良いことです。
     非形式的なものは人間とのコミュニケーションのために、
     形式的なものは実装と証明のためにです。 *)
 
-
 (* ####################################################### *)
-(* ** Evaluation *)
-(** ** 評価 *)
+(** ** Evaluation *)
 
-(* _Evaluating_ an arithmetic expression reduces it to a single number. *)
+(* _Evaluating_ an arithmetic expression produces a number. *)
 (** 算術式を評価する(_evaluating_)とその式を1つの数に簡約します。 *)
 
-Fixpoint aeval (e : aexp) : nat :=
-  match e with
+Fixpoint aeval (a : aexp) : nat :=
+  match a with
   | ANum n => n
   | APlus a1 a2 => (aeval a1) + (aeval a2)
   | AMinus a1 a2  => (aeval a1) - (aeval a2)
@@ -220,8 +195,8 @@ Proof. reflexivity. Qed.
 (* Similarly, evaluating a boolean expression yields a boolean. *)
 (** 同様に、ブール式を評価するとブール値になります。*)
 
-Fixpoint beval (e : bexp) : bool :=
-  match e with
+Fixpoint beval (b : bexp) : bool :=
+  match b with
   | BTrue       => true
   | BFalse      => false
   | BEq a1 a2   => beq_nat (aeval a1) (aeval a2)
@@ -243,8 +218,8 @@ Fixpoint beval (e : bexp) : bool :=
     算術式をとって、それを少し簡単化する関数を定義するとします。
     すべての [0+e] (つまり [(APlus (ANum 0) e)])を単に[e]にするものです。 *)
 
-Fixpoint optimize_0plus (e:aexp) : aexp :=
-  match e with
+Fixpoint optimize_0plus (a:aexp) : aexp :=
+  match a with
   | ANum n =>
       ANum n
   | APlus (ANum 0) e2 =>
@@ -276,48 +251,47 @@ Proof. reflexivity. Qed.
     -- つまり、最適化した式がオリジナルの式と同じ評価結果を返すことを確認したいならば、
     証明すべきです。 *)
 
-Theorem optimize_0plus_sound: forall e,
-  aeval (optimize_0plus e) = aeval e.
+Theorem optimize_0plus_sound: forall a,
+  aeval (optimize_0plus a) = aeval a.
 Proof.
-  intros e. induction e.
+  intros a. induction a.
   Case "ANum". reflexivity.
-  Case "APlus". destruct e1.
-    SCase "e1 = ANum n". destruct n.
-      SSCase "n = 0".  simpl. apply IHe2.
-      SSCase "n <> 0". simpl. rewrite IHe2. reflexivity.
-    SCase "e1 = APlus e1_1 e1_2".
-      simpl. simpl in IHe1. rewrite IHe1.
-      rewrite IHe2. reflexivity.
-    SCase "e1 = AMinus e1_1 e1_2".
-      simpl. simpl in IHe1. rewrite IHe1.
-      rewrite IHe2. reflexivity.
-    SCase "e1 = AMult e1_1 e1_2".
-      simpl. simpl in IHe1. rewrite IHe1.
-      rewrite IHe2. reflexivity.
+  Case "APlus". destruct a1.
+    SCase "a1 = ANum n". destruct n.
+      SSCase "n = 0".  simpl. apply IHa2.
+      SSCase "n <> 0". simpl. rewrite IHa2. reflexivity.
+    SCase "a1 = APlus a1_1 a1_2".
+      simpl. simpl in IHa1. rewrite IHa1.
+      rewrite IHa2. reflexivity.
+    SCase "a1 = AMinus a1_1 a1_2".
+      simpl. simpl in IHa1. rewrite IHa1.
+      rewrite IHa2. reflexivity.
+    SCase "a1 = AMult a1_1 a1_2".
+      simpl. simpl in IHa1. rewrite IHa1.
+      rewrite IHa2. reflexivity.
   Case "AMinus".
-    simpl. rewrite IHe1. rewrite IHe2. reflexivity.
+    simpl. rewrite IHa1. rewrite IHa2. reflexivity.
   Case "AMult".
-    simpl. rewrite IHe1. rewrite IHe2. reflexivity.  Qed.
+    simpl. rewrite IHa1. rewrite IHa2. reflexivity.  Qed.
 
 (* ####################################################### *)
 (* * Coq Automation *)
 (** * Coq の自動化 *)
 
 (* The repetition in this last proof is starting to be a little
-    annoying.  It's still just about bearable, but if either the
-    language of arithmetic expressions or the optimization being
-    proved sound were significantly more complex, it would begin to be
-    a real problem.
+    annoying.  If either the language of arithmetic expressions or the
+    optimization being proved sound were significantly more complex,
+    it would begin to be a real problem.
 
     So far, we've been doing all our proofs using just a small handful
-    of Coq's tactics and completely ignoring its very powerful
-    facilities for constructing proofs automatically.  This section
+    of Coq's tactics and completely ignoring its powerful facilities
+    for constructing parts of proofs automatically.  This section
     introduces some of these facilities, and we will see more over the
     next several chapters.  Getting used to them will take some
-    energy -- Coq's automation is a power tool -- but it will allow us to
-    scale up our efforts to more complex definitions and more
+    energy -- Coq's automation is a power tool -- but it will allow us
+    to scale up our efforts to more complex definitions and more
     interesting properties without becoming overwhelmed by boring,
-    repetitive, or low-level details. *)
+    repetitive, low-level details. *)
 (** 前の証明の最後の繰り返しはちょっと面倒です。今のところまだ耐えられますが、
     証明対象の言語や算術式や最適化が今に比べて著しく複雑だったら、現実的に問題になるでしょう。
 
@@ -335,89 +309,100 @@ Proof.
 (* ** Tacticals *)
 (** ** タクティカル(Tacticals) *)
 
-(* _Tactical_ is Coq's term for tactics that take other tactics as
+(* _Tacticals_ is Coq's term for tactics that take other tactics as
     arguments -- "higher-order tactics," if you will.  *)
 (** タクティカル(_tactical_)は Coq の用語で、
     他のタクティックを引数に取るタクティックのことです。
     「高階タクティック」("higher-order tactics")と言っても良いでしょう。 *)
 
 (* ####################################################### *)
-(* *** The [try] Tactical *)
-(** *** [try]タクティカル *)
+(* *** The [repeat] Tactical *)
+(** *** [repeat] タクティカル *)
 
-(* One very simple tactical is [try]: If [T] is a tactic, then [try
-    T] is a tactic that is just like [T] except that, if [T] fails,
-    [try T] does nothing at all (instead of failing). *)
-(** 非常にシンプルなタクティカルの1つが[try]です。[T]がタクティックのとき、
-    タクティック [try T] は[T]と同様ですが、[T]が失敗するとき
-    [try T] は(失敗せずに)何もしない点が違います。 *)
+(* The [repeat] tactical takes another tactic and keeps applying
+    this tactic until the tactic fails. Here is an example showing
+    that [100] is even using repeat. *)
+(** [repeat]タクティカルは、別のタクティックを引数として取り、そのタクティックが失敗するまで適用を続けます。以下は、repeatを使用した[100]が偶数であることをの証明の例です。*)
 
+Theorem ev100 : ev 100.
+Proof.
+  repeat (apply ev_SS). (* applies ev_SS 50 times,
+                           until [apply ev_SS] fails *)
+  apply ev_0.
+Qed.
+(* Print ev100. *)
+
+(** The [repeat T] tactic never fails; if the tactic [T] doesn't apply
+    to the original goal, then repeat still succeeds without changing
+    the original goal (it repeats zero times). *)
+(** [repeat T]タクティックは決して失敗しません。もし、タクティック[T]が現在のゴールに適用できない場合、ゴールを変更することなく、成功するまで繰り返します。(つまり0回繰り返します。*)
+Theorem ev100' : ev 100.
+Proof.
+  repeat (apply ev_0). (* doesn't fail, applies ev_0 zero times *)
+  (* 失敗はしません。ev_0が0回適用されます *)
+  repeat (apply ev_SS). apply ev_0. (* we can continue the proof *)
+  (* 証明を続行します。 *)
+Qed.
+
+(** The [repeat T] tactic does not have any bound on the number of
+    times it applies [T]. If [T] is a tactic that always succeeds then
+    repeat [T] will loop forever (e.g. [repeat simpl] loops forever
+    since [simpl] always succeeds). While Coq's term language is
+    guaranteed to terminate, Coq's tactic language is not! *)
+(** [repeat T]タクティックは、[T]を適用する回数の限界値について関知しません。
+もし、[T]が常に成功する場合、[T]を永久に繰り返します。(例えば、[repeat simpl]は
+[simpl]が常に成功するため、無限ループします。) Coqは自身の言語については、終了を保証していますが、Coqのタクティック言語については、そうではないのです。*)
 (* ####################################################### *)
-(* *** The [;] Tactical *)
-(** *** [;]タクティカル *)
+(** *** The [try] Tactical *)
 
-(* Another very basic tactical is written [;].  If [T], [T1], ...,
-    [Tn] are tactics, then
-[[
-      T; [T1 | T2 | ... | Tn]
-]]
-   is a tactic that first performs [T] and then performs [T1] on the
-   first subgoal generated by [T], performs [T2] on the second
-   subgoal, etc.
+(** If [T] is a tactic, then [try T] is a tactic that is just like [T]
+    except that, if [T] fails, [try T] _successfully_ does nothing at
+    all (instead of failing). *)
+(** [T]がタクティックのとき、タクティック [try T] は[T]と同様ですが、[T]が失敗するとき[try T] は(失敗せずに)何もしない点が違います。 *)
 
-   In the special case where all of the [Ti]'s are the same tactic
-   [T'], we can just write [T;T'] instead of:
-[[
-      T; [T' | T' | ... | T']
-]]
-   That is, if [T] and [T'] are tactics, then [T;T'] is a tactic that
-   first performs [T] and then performs [T'] on _each subgoal_
-   generated by [T].  This is the form of [;] that is used most often
-   in practice. *)
-(** 別の非常に基本的なタクティカルは[;]と書かれます。
-    [T], [T1], ..., [Tn] がタクティックのとき、
-[[
-      T; [T1 | T2 | ... | Tn]
-]]
-   はタクティックで、最初に[T]を行ない、
-   [T]によって生成された最初のサブゴールに[T1]を行ない、
-   二番目のサブゴールに[T2]を行ない、... という処理をします。
+Theorem silly1 : forall ae, aeval ae = aeval ae.
+Proof. try reflexivity. (* this just does [reflexivity] *) Qed.
 
-   すべての[Ti]が同じタクティック[T']であるという特別な場合、
-[[
-      T; [T' | T' | ... | T']
-]]
-   と書く代わりに [T;T'] と書くだけで済ますことができます。
-   つまり、[T]と[T']がタクティックのとき、
-   [T;T'] はタクティックで、最初に[T]を行ない、
-   [T]が生成したそれぞれのサブゴールに[T']を行ないます。
-   これが[;]の実際に一番よく使われる形です。*)
+Theorem silly2 : forall (P : Prop), P -> P.
+Proof.
+  intros P HP.
+  try reflexivity. (* just [reflexivity] would have failed *)
+  apply HP. (* we can still finish the proof in some other way *)
+Qed.
 
+(* Using [try] in a completely manual proof is a bit silly, but
+    we'll see below that [try] is very useful for doing automated
+    proofs in conjunction with the [;] tactical. *)
+(** [try]タクティックを手動の証明で使用することは少し馬鹿げていると思われるかもしれまんが、こみいった自動化された証明において、[;]と同時に使用することで非常に便利になります *)
+(* ####################################################### *)
+(* *** The [;] Tactical (Simple Form) *)
+(** *** [;]タクティカル(単純な形式) *)
+
+(* In its most commonly used form, the [;] tactical takes two tactics
+    as argument: [T;T'] first performs the tactic [T] and then
+    performs the tactic [T'] on _each subgoal_ generated by [T]. *)
+(** [;]が最も使用されるのは、[T;T']ように、二つのタクティックを引数にとるやりかたです。最初にタクティック[T]が実行され、次にタクティック[T']が[T]によって生成された、それぞれのサブゴールにおいて実行されます。*)
 (* For example, consider the following trivial lemma: *)
-(** 例えば、次の簡単な補題を考えます: *)
+(** 例として、次のちょっとした補題について考えてみましょう: *)
 
 Lemma foo : forall n, ble_nat 0 n = true.
 Proof.
   intros.
   destruct n.
-    (* Leaves two subgoals...  *)
+    (* Leaves two subgoals, which are discharged identically...  *)
     Case "n=0". simpl. reflexivity.
     Case "n=Sn'". simpl. reflexivity.
-    (* ... which are discharged similarly *)
 Qed.
 
-(* We can simplify the proof above using the [;] tactical. *)
-(** 上の証明を[;]タクティカルを使って簡単化できます。 *)
+(* We can simplify this proof using the [;] tactical: *)
+(** [;] タクティカルを使用することで証明がシンプルになります。: *)
 
 Lemma foo' : forall n, ble_nat 0 n = true.
 Proof.
   intros.
-  (* Apply [destruct] to the current goal *)
-  destruct n;
-  (* then apply [simpl] to each resulting subgoal *)
-  simpl;
-  (* then apply [reflexivity] to each resulting subgoal *)
-  reflexivity.
+  destruct n; (* [destruct] the current goal *)
+  simpl; (* then [simpl] each resulting subgoal *)
+  reflexivity. (* and do [reflexivity] on each resulting subgoal *)
 Qed.
 
 (* Using [try] and [;] together, we can get rid of the repetition in
@@ -425,91 +410,80 @@ Qed.
 (** [try]と[;]の両方を使うと、
     ちょっと前に悩まされた証明の繰り返しを取り除くことができます。 *)
 
-Theorem optimize_0plus_sound': forall e,
-  aeval (optimize_0plus e) = aeval e.
+Theorem optimize_0plus_sound': forall a,
+  aeval (optimize_0plus a) = aeval a.
 Proof.
-  intros e.
-  induction e;
+  intros a.
+  induction a;
     (* Most cases follow directly by the IH *)
-    try (simpl; rewrite IHe1; rewrite IHe2; reflexivity).
+    try (simpl; rewrite IHa1; rewrite IHa2; reflexivity).
+  (* The remaining cases -- ANum and APlus -- are different *)
   Case "ANum". reflexivity.
   Case "APlus".
-    destruct e1;
-      (* Most cases follow directly by the IH *)
-      try (simpl; simpl in IHe1; rewrite IHe1; rewrite IHe2; reflexivity).
-    (* The interesting case, on which the above fails, is
-       when [e1 = ANum n]. In this case, we have to destruct [n]
-       (to see whether the optimization applies) and rewrite
+    destruct a1;
+      (* Again, most cases follow directly by the IH *)
+      try (simpl; simpl in IHa1; rewrite IHa1;
+           rewrite IHa2; reflexivity).
+    (* The interesting case, on which the [try...] does nothing,
+       is when [e1 = ANum n]. In this case, we have to destruct
+       [n] (to see whether the optimization applies) and rewrite
        with the induction hypothesis. *)
-    SCase "e1 = ANum n". destruct n;
-      simpl; rewrite IHe2; reflexivity.   Qed.
+    SCase "a1 = ANum n". destruct n;
+      simpl; rewrite IHa2; reflexivity.   Qed.
 
-(* In practice, Coq experts often use [try] with a tactic like
-    [induction] to take care of many similar "straightforward" cases
-    all at once.  Naturally, this practice has an analog in informal
-    proofs. *)
-(** 実際的にはCoqの専門家は、[try]を[induction]のようなタクティックと一緒に使うことで、
-    多くの似たような「簡単な」場合を一度に処理します。
-    これは自然に非形式的な証明に対応します。*)
-(* Here is an informal proof of this theorem that
-    matches the structure of the formal one:
+(* Coq experts often use this "[...; try... ]" idiom after a tactic
+    like [induction] to take care of many similar cases all at once.
+    Naturally, this practice has an analog in informal proofs.
 
-    _Theorem_: For all arithmetic expressions [e],
-[[
-       aeval (optimize_0plus e) = aeval e.
-]]
-    _Proof_: By induction on [e].  The [AMinus] and [AMult] cases
+    Here is an informal proof of this theorem that matches the
+    structure of the formal one: 
+
+    _Theorem_: For all arithmetic expressions [a],
+       aeval (optimize_0plus a) = aeval a.
+    _Proof_: By induction on [a].  The [AMinus] and [AMult] cases
     follow directly from the IH.  The remaining cases are as follows:
 
-      - Suppose [e = ANum n] for some [n].  We must show
-[[
+      - Suppose [a = ANum n] for some [n].  We must show
           aeval (optimize_0plus (ANum n)) = aeval (ANum n).
-]]
         This is immediate from the definition of [optimize_0plus].
 
-      - Suppose [e = APlus e1 e2] for some [e1] and [e2].  We
+      - Suppose [a = APlus a1 a2] for some [a1] and [a2].  We
         must show
-[[
-          aeval (optimize_0plus (APlus e1 e2))
-        = aeval (APlus e1 e2).
-]]
-        Consider the possible forms of [e1].  For most of them,
+          aeval (optimize_0plus (APlus a1 a2))
+        = aeval (APlus a1 a2).
+        Consider the possible forms of [a1].  For most of them,
         [optimize_0plus] simply calls itself recursively for the
         subexpressions and rebuilds a new expression of the same form
-        as [e1]; in these cases, the result follows directly from the
+        as [a1]; in these cases, the result follows directly from the
         IH.
 
-        The interesting case is when [e1 = ANum n] for some [n].
+        The interesting case is when [a1 = ANum n] for some [n].
         If [n = ANum 0], then
-[[
-          optimize_0plus (APlus e1 e2) = optimize_0plus e2
-]]
-        and the IH for [e2] is exactly what we need.  On the other
+          optimize_0plus (APlus a1 a2) = optimize_0plus a2
+        and the IH for [a2] is exactly what we need.  On the other
         hand, if [n = S n'] for some [n'], then again [optimize_0plus]
         simply calls itself recursively, and the result follows from
         the IH.  [] *)
-(** この定理の形式的な証明の構造にマッチする非形式的な証明は次の通りです:
+(** 実際的にはCoqの専門家は、[try]を[induction]のようなタクティックと一緒に使うことで、
+    多くの似たような「簡単な」場合を一度に処理します。
+    これは自然に非形式的な証明に対応します。
+
+    この定理の形式的な証明の構造にマッチする非形式的な証明は次の通りです:
 
     「定理」: すべての算術式[e]について
-[[
        aeval (optimize_0plus e) = aeval e.
-]]
     「証明」: [e]についての帰納法を使う。
     [AMinus]と[AMult]の場合は帰納仮定から直接得られる。
     残るのは以下の場合である:
 
       - ある[n]について [e = ANum n] とする。示すべきことは次の通りである:
-[[
           aeval (optimize_0plus (ANum n)) = aeval (ANum n).
-]]
         これは[optimize_0plus]の定義からすぐに得られる。
 
       - ある[e1]と[e2]について [e = APlus e1 e2] とする。
         示すべきことは次の通りである:
-[[
           aeval (optimize_0plus (APlus e1 e2))
         = aeval (APlus e1 e2).
-]]
         [e1]のとり得る形を考える。そのほとんどの場合、
         [optimize_0plus]は部分式について単に自分自身を再帰的に呼び出し、
         [e1]と同じ形の新しい式を再構成する。
@@ -517,15 +491,13 @@ Proof.
 
         興味深い場合は、ある[n]について [e1 = ANum n] であるときである。
         このとき [n = ANum 0] ならば次が成立する:
-[[
           optimize_0plus (APlus e1 e2) = optimize_0plus e2
-]]
         そして[e2]についての帰納仮定がまさに求めるものである。
         一方、ある[n']について [n = S n'] ならば、
         [optimize_0plus]はやはり自分自身を再帰的に呼び出し、
         結果は帰納仮定から得られる。 [] *)
 
-(* This proof can still be improved: the first case (for [e = ANum
+(** This proof can still be improved: the first case (for [a = ANum
     n]) is very trivial -- even more trivial than the cases that we
     said simply followed from the IH -- yet we have chosen to write it
     out in full.  It would be better and clearer to drop it and just
@@ -541,21 +513,46 @@ Proof.
     と言った方がより良く、より明快でしょう。
     同じ改良を形式的な証明にも行うことができます。以下のようになります: *)
 
-Theorem optimize_0plus_sound'': forall e,
-  aeval (optimize_0plus e) = aeval e.
+Theorem optimize_0plus_sound'': forall a,
+  aeval (optimize_0plus a) = aeval a.
 Proof.
-  intros e.
-  induction e;
+  intros a.
+  induction a;
     (* Most cases follow directly by the IH *)
-    try (simpl; rewrite IHe1; rewrite IHe2; reflexivity);
+    try (simpl; rewrite IHa1; rewrite IHa2; reflexivity);
     (* ... or are immediate by definition *)
     try reflexivity.
-  (* The interesting case is when e = APlus e1 e2. *)
+  (* The interesting case is when a = APlus a1 a2. *)
   Case "APlus".
-    destruct e1; try (simpl; simpl in IHe1; rewrite IHe1;
-                      rewrite IHe2; reflexivity).
-    SCase "e1 = ANum n". destruct n;
-      simpl; rewrite IHe2; reflexivity.  Qed.
+    destruct a1; try (simpl; simpl in IHa1; rewrite IHa1;
+                      rewrite IHa2; reflexivity).
+    SCase "a1 = ANum n". destruct n;
+      simpl; rewrite IHa2; reflexivity. Qed.
+
+(* ####################################################### *)
+(* *** The [;] Tactical (General Form) *)
+(** *** [;] タクティカル (一般的な形式) *)
+
+(* The [;] tactical has a more general than the simple [T;T'] we've
+    seen above, which is sometimes also useful.  If [T], [T1], ...,
+    [Tn] are tactics, then
+      T; [T1 | T2 | ... | Tn]
+   is a tactic that first performs [T] and then performs [T1] on the
+   first subgoal generated by [T], performs [T2] on the second
+   subgoal, etc.
+
+   So [T;T'] is just special notation for the case when all of the
+   [Ti]'s are the same tactic; i.e. [T;T'] is just a shorthand for:
+      T; [T' | T' | ... | T']
+*)
+(** 上記で見た、単純な、[T;T']よりも一般的に[;]を使うことが出来、しぱしば有用です。[T],[T1],...,[Tn]がタクティカルならば、
+    T; [T1| T2 | ... | Tn]
+   はタクティックで、最初に[T]を行ない、
+   [T]によって生成された最初のサブゴールに[T1]を行ない、
+   二番目のサブゴールに[T2]を行ない、... という処理をします。 
+   すべての[Ti]が同じタクティック[T']であるという特別な場合、
+      T; [T' | T' | ... | T']
+   と書く代わりに [T;T'] と書くだけで済ますことができます。*)
 
 (* ####################################################### *)
 (* ** Defining New Tactic Notations *)
@@ -563,9 +560,9 @@ Proof.
 
 (* Coq also provides several ways of "programming" tactic scripts.
 
-      - The [Tactic Notation] command gives a handy way to define
-        "shorthand tactics" that, when invoked, apply several tactics
-        at the same time.
+      - The [Tactic Notation] idiom illustrated below gives a handy
+        way to define "shorthand tactics" that bundle several tactics
+        into a single command.
 
       - For more sophisticated programming, Coq offers a small
         built-in programming language called [Ltac] with primitives
@@ -576,10 +573,9 @@ Proof.
         there are many examples of [Ltac] definitions in the Coq
         standard library that you can use as examples.
 
-      - There is also an OCaml API that can be used to build new
-        tactics that access Coq's internal structures at a lower
-        level, but this is seldom worth the trouble for ordinary Coq
-        users.
+      - There is also an OCaml API, which can be used to build tactics
+        that access Coq's internal structures at a lower level, but
+        this is seldom worth the trouble for ordinary Coq users.
 
 The [Tactic Notation] mechanism is the easiest to come to grips with,
 and it offers plenty of power for many purposes.  Here's an example.
@@ -629,8 +625,8 @@ Tactic Notation "simpl_and_try" tactic(c) :=
 (* *** Bulletproofing Case Analyses *)
 (** *** 場合分けを万全にする *)
 
-(* Being able to deal with most of the cases of an [induction] or
-    [destruct] all at the same time is very convenient, but it can
+(** Being able to deal with most of the cases of an [induction]
+    or [destruct] all at the same time is very convenient, but it can
     also be a little confusing.  One problem that often comes up is
     that _maintaining_ proofs written in this style can be difficult.
     For example, suppose that, later, we extended the definition of
@@ -641,8 +637,8 @@ Tactic Notation "simpl_and_try" tactic(c) :=
     actually expecting the argument for a completely different
     constructor.  What we'd like is to get a sensible error message
     saying "I was expecting the [AFoo] case at this point, but the
-    proof script is talking about [APlus]."  Here's a nice little
-    trick that smoothly achieves this. *)
+    proof script is talking about [APlus]."  Here's a nice trick (due
+    to Aaron Bohannon) that smoothly achieves this. *)
 (** [induction]や[destruct]で、ほとんどの場合を一度に扱えるのはとても便利ですが、
     またちょっと混乱もします。よく起こる問題は、
     このスタイルで記述された証明をメンテナンスすることが難しいということです。
@@ -668,48 +664,47 @@ Tactic Notation "aexp_cases" tactic(first) ident(c) :=
 (** ([Case_aux]は[Case]、[SCase]、[SSCase]等の共通機能を実装します。
     例えば、[Case "foo"]は [Case_aux Case "foo"] と定義されます。) *)
 
-(* For example, if [e] is a variable of type [aexp], then doing
-[[
-      aexp_cases (induction e) Case
-]]
-    will perform an induction on [e] (the same as if we had just typed
-    [induction e]) and _also_ add a [Case] tag to each subgoal
+(* For example, if [a] is a variable of type [aexp], then doing
+      aexp_cases (induction a) Case
+    will perform an induction on [a] (the same as if we had just typed
+    [induction a]) and _also_ add a [Case] tag to each subgoal
     generated by the [induction], labeling which constructor it comes
     from.  For example, here is yet another proof of
-    optimize_0plus_sound, using [aexp_cases]: *)
+    [optimize_0plus_sound], using [aexp_cases]: *)
 (** 例えば、[e]が型[aexp]の変数のとき、
-[[
       aexp_cases (induction e) Case
-]]
     と書くと[e]についての帰納法を実行し(単に [induction e] と書いたのと同じです)、
     そして、「その上に」、[induction]によって生成されたそれぞれのサブゴールに[Case]
     タグを付加します。このタグは、そのサブゴールがどのコンストラクタから来たかのラベルです。
     例えば、[aexp_cases]を使った、[optimize_0plus_sound]のさらに別証です: *)
 
-Theorem optimize_0plus_sound''': forall e,
-  aeval (optimize_0plus e) = aeval e.
+Theorem optimize_0plus_sound''': forall a,
+  aeval (optimize_0plus a) = aeval a.
 Proof.
-  intros e.
-  aexp_cases (induction e) Case;
-    try (simpl; rewrite IHe1; rewrite IHe2; reflexivity);
+  intros a.
+  aexp_cases (induction a) Case;
+    try (simpl; rewrite IHa1; rewrite IHa2; reflexivity);
     try reflexivity.
-
-  (* At this point, there is already an ["APlus"] case name in the
-     context.  The [Case "APlus"] here in the proof text has the
-     effect of a sanity check: if the "Case" string in the context is
-     anything _other_ than ["APlus"] (for example, because we added a
-     clause to the definition of [aexp] and forgot to change the
-     proof) we'll get a helpful error at this point telling us that
-     this is now the wrong case. *)
+  (* At this point, there is already an ["APlus"] case name
+     in the context.  The [Case "APlus"] here in the proof
+     text has the effect of a sanity check: if the "Case"
+     string in the context is anything _other_ than ["APlus"]
+     (for example, because we added a clause to the definition
+     of [aexp] and forgot to change the proof) we'll get a
+     helpful error at this point telling us that this is now
+     the wrong case. *)
+  (* この時点で、すでに["APlus"]の名前はコンテキストに導入されています。
+  [Case "Aplus"]のテキストは証明のこの時点で健全性のチェックの効果を持ちます。
+  ：もし、コンテキスト中の"Case"文字列が["APlus"]ではない他のものである場合、(例えば、[aexp]に後から追加されていたにも係らず、証明の変更を忘れていたなど)ここで場合分けが間違っていることに気が付くことが出来ます。*)
   Case "APlus".
-    aexp_cases (destruct e1) SCase;
-      try (simpl; simpl in IHe1; rewrite IHe1; rewrite IHe2; reflexivity).
+    aexp_cases (destruct a1) SCase;
+      try (simpl; simpl in IHa1;
+           rewrite IHa1; rewrite IHa2; reflexivity).
     SCase "ANum". destruct n;
-      simpl; rewrite IHe2; reflexivity.  Qed.
+      simpl; rewrite IHa2; reflexivity.  Qed.
 
-(* **** Exercise: 3 stars (optimize_0plus_b) *)
-(** **** 練習問題: ★★★ (optimize_0plus_b) *)
-(* Since the [optimize_0plus] tranformation doesn't change the value
+(** **** Exercise: 3 stars (optimize_0plus_b) *)
+(** Since the [optimize_0plus] tranformation doesn't change the value
     of [aexp]s, we should be able to apply it to all the [aexp]s that
     appear in a [bexp] without changing the [bexp]'s value.  Write a
     function which performs that transformation on [bexp]s, and prove
@@ -722,12 +717,18 @@ Proof.
     それが健全であることを証明しなさい。
     ここまで見てきたタクティカルを使って証明を可能な限りエレガントにしなさい。*)
 
-(* FILL IN HERE *)
+Fixpoint optimize_0plus_b (b : bexp) : bexp :=
+  (* FILL IN HERE *) admit.
+
+
+Theorem optimize_0plus_b_sound : forall b,
+  beval (optimize_0plus_b b) = beval b.
+Proof.
+  (* FILL IN HERE *) Admitted.
 (** [] *)
 
-(* **** Exercise: 4 stars, optional (optimizer) *)
-(** **** 練習問題: ★★★★, optional (optimizer) *)
-(* _Design exercise_: The optimization implemented by our
+(** **** Exercise: 4 stars, optional (optimizer) *)
+(** _Design exercise_: The optimization implemented by our
     [optimize_0plus] function is only one of many imaginable
     optimizations on arithmetic and boolean expressions.  Write a more
     sophisticated optimizer and prove it correct.
@@ -786,14 +787,16 @@ Proof.
   intros. omega.
 Qed.
 
-(* Andrew Appel calls this the "Santa Claus tactic." *)
-(** Andrew Appel は[omega]を「サンタクロース・タクティック」と呼んでいます。 *)
-
+(** Liebniz wrote, "It is unworthy of excellent men to lose
+    hours like slaves in the labor of calculation which could be
+    relegated to anyone else if machines were used."  We recommend
+    using the omega tactic whenever possible. *)
+(** "優れた人間が奴隷に格下げになるような機械でも出来るような誰でも出来る計算に従事して時間を無駄にすることほど勿体ないことはない。"とライプニッツは書いています。*)
 (* ####################################################### *)
 (* ** A Few More Handy Tactics *)
 (** ** 便利なタクティックをさらにいくつか *)
 
-(* Finally, here are some miscellaneous tactics that you may find
+(** Finally, here are some miscellaneous tactics that you may find
     convenient.
 
      - [clear H]: Delete hypothesis [H] from the context.
@@ -815,15 +818,14 @@ Qed.
        [apply H].
 
      - [contradiction]: Try to find a hypothesis [H] in the current
-       context that is equivalent to [False].  If one is found, solve
-       the goal.
+       context that is logically equivalent to [False].  If one is
+       found, solve the goal.
 
      - [constructor]: Try to find a constructor [c] (from some
        [Inductive] definition in the current environment) that can be
        applied to solve the current goal.  If one is found, behave
-       like [apply c].
+       like [apply c]. *)
 
-    We'll see many examples of these in the proofs below. *)
 (** 最後に、役に立ちそうないろいろなタクティックをいくつか紹介します。
 
      - [clear H]: 仮定[H]をコンテキストから消去します。
@@ -846,25 +848,27 @@ Qed.
 
      - [constructor]: 現在のゴールを解くのに使えるコンストラクタ[c]を
        (現在の環境の[Inductive]による定義から)探そうとします。
-       発見されたときは [apply c] と同様に振る舞います。
+       発見されたときは [apply c] と同様に振る舞います。 *)
 
-    以降の証明でこれらのたくさんの例を見るでしょう。 *)
+(* We'll see many examples of these in the proofs below. *)
+(** 以降の証明でこれらのたくさんの例を見るでしょう。 *)
 
 (* ####################################################### *)
 (* * Evaluation as a Relation *)
 (** * 関係としての評価 *)
 
 (* We have presented [aeval] and [beval] as functions defined by
-    [Fixpoints]. An alternative way to think about evaluation is as a
-    _relation_ between expressions and their values.
-
-    This leads naturally to Coq [Inductive] definitions like the
-    following one for arithmetic expressions... *)
+    [Fixpoints].  Another way to think about evaluation -- one that we
+    will see is often more flexible -- is as a _relation_ between
+    expressions and their values.  This leads naturally to [Inductive]
+    definitions like the following one for arithmetic
+    expressions... *)
 (** [aeval]と[beval]を[Fixpoints]によって定義された関数として示しました。
     評価について考える別の方法は、それを式と値との間の関係(_relation_)と見ることです。
 
     この考えに立つと、
     算術式についてCoqの[Inductive]による以下の定義が自然に出てきます... *)
+
 
 Module aevalR_first_try.
 
@@ -884,14 +888,14 @@ Inductive aevalR : aexp -> nat -> Prop :=
       aevalR e2 n2 ->
       aevalR (AMult e1 e2) (n1 * n2).
 
-(* As is often the case with relations, we'll find it
+(** As is often the case with relations, we'll find it
     convenient to define infix notation for [aevalR].  We'll write [e
     || n] to mean that arithmetic expression [e] evaluates to value
-    [n].  (This notation is one place where the limitation to ascii
+    [n].  (This notation is one place where the limitation to ASCII
     symbols becomes a little bothersome.  The standard notation for
     the evaluation relation is a double down-arrow.  We'll typeset it
     like this in the HTML version of the notes and use a double
-    vertical bar as the closest approximation in ascii .v files.)  *)
+    vertical bar as the closest approximation in [.v] files.)  *)
 (** 関係についてよく行うように、[aevalR]の中置記法を定義するのが便利です。
     算術式[e]が値[n]に評価されることを [e || n] と書きます。
     (この記法は煩わしいascii記号の限界の1つです。評価関係の標準記法は二重の下向き矢印です。
@@ -936,11 +940,112 @@ Tactic Notation "aevalR_cases" tactic(first) ident(c) :=
   [ Case_aux c "E_ANum" | Case_aux c "E_APlus"
   | Case_aux c "E_AMinus" | Case_aux c "E_AMult" ].
 
-(* It is straightforward to prove that the relational and functional
+(* ####################################################### *)
+(* ** Inference Rule Notation *)
+(** ** 推論規則記法 *)
+
+(* In informal discussions, it is convenient write the rules for
+    [aevalR] and similar relations in the more readable graphical form
+    of _inference rules_, where the premises above the line justify
+    the conclusion below the line (we have already seen them in the
+    Prop chapter). *)
+(** 非形式的な議論には、[aevalR]や似たような関係についての規則を、
+    推論規則(_inference rules_)と呼ばれる、
+    より読みやすいグラフィカルな形で書くのが便利です。
+    推論規則は、横線の上の前提から、横線の下の結論を導出できることを述べます。
+	( すでに、Propの章で見ていると思います。)
+
+(* For example, the constructor [E_APlus]...
+      | E_APlus : forall (e1 e2: aexp) (n1 n2: nat),
+          aevalR e1 n1 ->
+          aevalR e2 n2 ->
+          aevalR (APlus e1 e2) (n1 + n2)
+    ...would be written like this as an inference rule:
+                               e1 || n1
+                               e2 || n2
+                         --------------------                         (E_APlus)
+                         APlus e1 e2 || n1+n2
+*)
+(** 例えば、コンストラクタ[E_APlus]...
+      | E_APlus : forall (e1 e2: aexp) (n1 n2: nat),
+          aevalR e1 n1 ->
+          aevalR e2 n2 ->
+          aevalR (APlus e1 e2) (n1 + n2)
+    ...は推論規則として次のように書けるでしょう:
+                               e1 || n1
+                               e2 || n2
+                         --------------------                         (E_APlus)
+                         APlus e1 e2 || n1+n2
+*)
+(* Formally, there is nothing very deep about inference rules:
+    they are just implications.  You can read the rule name on the
+    right as the name of the constructor and read each of the
+    linebreaks between the premises above the line and the line itself
+    as [->].  All the variables mentioned in the rule ([e1], [n1],
+    etc.) are implicitly bound by universal quantifiers at the
+    beginning. (Such variables are often called _metavariables_ to
+    distinguish them from the variables of the language we are
+    defining.  At the moment, our arithmetic expressions don't include
+    variables, but we'll soon be adding them.)  The whole collection
+    of rules is understood as being wrapped in an [Inductive]
+    declaration (informally, this is either elided or else indicated
+    by saying something like "Let [aevalR] be the smallest relation
+    closed under the following rules..."). *)
+(** 形式的には、推論規則について何も深いものはありません。単なる含意です。
+    右に書かれた規則名はコンストラクタで、
+    横線より上の前提の間の各改行と横線自体は[->]と読むことができます。
+    規則で言及されるすべての変数([e1]、[n1]等)
+    は暗黙のうちに冒頭で全称限量子に束縛されています。
+    規則の集合全体は[Inductive]宣言で囲われていると理解されます
+    (これは完全に暗黙のまま置かれるか、非形式的に
+    「[aevalR]は以下の規則について閉じた最小の関係とします...」
+    などと述べられるかします)。 *)
+(* For example, [||] is the smallest relation closed under these
+    rules:
+                             -----------                               (E_ANum)
+                             ANum n || n
+
+                               e1 || n1
+                               e2 || n2
+                         --------------------                         (E_APlus)
+                         APlus e1 e2 || n1+n2
+
+                               e1 || n1
+                               e2 || n2
+                        ---------------------                        (E_AMinus)
+                        AMinus e1 e2 || n1-n2
+
+                               e1 || n1
+                               e2 || n2
+                         --------------------                         (E_AMult)
+                         AMult e1 e2 || n1*n2
+*)
+(** 例えば、[||]は以下の規則について閉じた最小の関係です:
+                             -----------                               (E_ANum)
+                             ANum n || n
+
+                               e1 || n1
+                               e2 || n2
+                         --------------------                         (E_APlus)
+                         APlus e1 e2 || n1+n2
+
+                               e1 || n1
+                               e2 || n2
+                        ---------------------                        (E_AMinus)
+                        AMinus e1 e2 || n1-n2
+
+                               e1 || n1
+                               e2 || n2
+                         --------------------                         (E_AMult)
+                         AMult e1 e2 || n1*n2
+*)
+
+(* ####################################################### *)
+(* ** Equivalence of the Definitions *)
+(** ** 等価性の定義 *)
+(** It is straightforward to prove that the relational and functional
     definitions of evaluation agree on all possible arithmetic
     expressions... *)
-(** 評価の、関係による定義と関数による定義が、
-    すべての算術式について一致することを証明するのは簡単です... *)
 
 Theorem aeval_iff_aevalR : forall a n,
   (a || n) <-> aeval a = n.
@@ -977,8 +1082,15 @@ Proof.
       apply IHa2. reflexivity.
 Qed.
 
-(* A shorter proof making more aggressive use of tacticals: *)
-(** タクティカルをより積極的に使ったより短い証明です: *)
+(** Note: if you're reading the HTML file, you'll see an empty square box instead
+of a proof for this theorem.  
+You can click on this box to "unfold" the text to see the proof.
+Click on the unfolded to text to "fold" it back up to a box. We'll be using
+this style frequently from now on to help keep the HTML easier to read.
+The full proofs always appear in the .v files. *)
+
+(** We can make the proof quite a bit shorter by making more
+    use of tacticals... *)
 
 Theorem aeval_iff_aevalR' : forall a n,
   (a || n) <-> aeval a = n.
@@ -993,175 +1105,116 @@ Proof.
        try apply IHa1; try apply IHa2; reflexivity.
 Qed.
 
-(* **** Exercise: 2 stars, optional (bevalR) *)
-(** **** 練習問題: ★★, optional (bevalR) *)
-(* Write a relation [bevalR] in the same style as
+(** **** Exercise: 3 stars  (bevalR) *)
+(** Write a relation [bevalR] in the same style as
     [aevalR], and prove that it is equivalent to [beval].*)
-(** 関係[bevalR]を[aevalR]と同じスタイルで記述し、
-    それが[beval]と同値であることを証明しなさい。 *)
 
-(*
+(* 
 Inductive bevalR:
 (* FILL IN HERE *)
+*)
 (** [] *)
-*)
-
-(* For the definitions of evaluation for arithmetic and boolean
-    expressions, the choice of whether to use functional or relational
-    definitions is mainly a matter of taste.  In general, Coq has
-    somewhat better support for working with relations; in particular,
-    we can more readily do induction over them.  On the other hand, in
-    some sense function definitions carry more information, because
-    functions are necessarily deterministic and defined on all
-    arguments; for a relation we have to show these properties
-    explicitly if we need them.
-
-    However, there are circumstances where relational definitions of
-    evaluation are greatly preferable to functional ones, as we'll see
-    shortly. *)
-(** 算術式とブール式の評価の定義について、関数を使うか関係を使うかはほとんど趣味の問題です。
-    一般に、Coqは関係を扱う方がいくらかサポートが厚いです。
-    特に帰納法についてはそうです。一方、
-    ある意味で関数による定義の方がより多くの情報を持っています。
-    なぜなら、関数は決定的でなければならず、
-    またすべての引数について定義されていなければなりません。
-    関数については、必要ならばこれらの性質を明示的に示さなければなりません。
-
-    しかしながら、評価の定義として、
-    関係による定義が関数による定義よりはるかに望ましい状況があります。
-    以下で簡単に見ます。 *)
-
-(* ####################################################### *)
-(* ** Inference Rule Notation *)
-(** ** 推論規則記法 *)
-
-(* In informal discussions, it is convenient write the rules for
-    [aevalR] and similar relations in a more readable "graphical" form
-    called _inference rules_, where the premises above the line allow
-    you to derive the conclusion below the line.  For example, the
-    constructor [E_APlus]...
-[[
-      | E_APlus : forall (e1 e2: aexp) (n1 n2: nat),
-          aevalR e1 n1 ->
-          aevalR e2 n2 ->
-          aevalR (APlus e1 e2) (n1 + n2)
-]]
-    ...would be written like this as an inference rule:
-[[[
-                               e1 || n1
-                               e2 || n2
-                         --------------------                         (E_APlus)
-                         APlus e1 e2 || n1+n2
-]]]
-    Formally, there is nothing very deep about inference rules: they
-    are just implications.  You can read the rule name on the right as
-    the name of the constructor and read each of the linebreaks
-    between the premises above the line and the line itself as [->].
-    All the variables mentioned in the rule ([e1], [n1], etc.) are
-    implicitly bound by universal quantifiers at the beginning.  The
-    whole collection of rules is understood as being wrapped in an
-    [Inductive] declaration (this is either left completely implicit
-    or else indicated informally by saying something like "Let
-    [aevalR] be the smallest relation closed under the following
-    rules...").
-
-    For example, [||] is the smallest relation closed under these
-    rules:
-[[[
-                             -----------                               (E_ANum)
-                             ANum n || n
-
-                               e1 || n1
-                               e2 || n2
-                         --------------------                         (E_APlus)
-                         APlus e1 e2 || n1+n2
-
-                               e1 || n1
-                               e2 || n2
-                        ---------------------                        (E_AMinus)
-                        AMinus e1 e2 || n1-n2
-
-                               e1 || n1
-                               e2 || n2
-                         --------------------                         (E_AMult)
-                         AMult e1 e2 || n1*n2
-]]]
-*)
-(** 非形式的な議論には、[aevalR]や似たような関係についての規則を、
-    推論規則(_inference rules_)と呼ばれる、
-    より読みやすいグラフィカルな形で書くのが便利です。
-    推論規則は、横線の上の前提から、横線の下の結論を導出できることを述べます。
-    例えば、コンストラクタ[E_APlus]...
-[[
-      | E_APlus : forall (e1 e2: aexp) (n1 n2: nat),
-          aevalR e1 n1 ->
-          aevalR e2 n2 ->
-          aevalR (APlus e1 e2) (n1 + n2)
-]]
-    ...は推論規則として次のように書けるでしょう:
-[[
-                               e1 || n1
-                               e2 || n2
-                         --------------------                         (E_APlus)
-                         APlus e1 e2 || n1+n2
-]]
-    形式的には、推論規則について何も深いものはありません。単なる含意です。
-    右に書かれた規則名はコンストラクタで、
-    横線より上の前提の間の各改行と横線自体は[->]と読むことができます。
-    規則で言及されるすべての変数([e1]、[n1]等)
-    は暗黙のうちに冒頭で全称限量子に束縛されています。
-    規則の集合全体は[Inductive]宣言で囲われていると理解されます
-    (これは完全に暗黙のまま置かれるか、非形式的に
-    「[aevalR]は以下の規則について閉じた最小の関係とします...」
-    などと述べられるかします)。
-
-    例えば、[||]は以下の規則について閉じた最小の関係です:
-[[
-                             -----------                               (E_ANum)
-                             ANum n || n
-
-                               e1 || n1
-                               e2 || n2
-                         --------------------                         (E_APlus)
-                         APlus e1 e2 || n1+n2
-
-                               e1 || n1
-                               e2 || n2
-                        ---------------------                        (E_AMinus)
-                        AMinus e1 e2 || n1-n2
-
-                               e1 || n1
-                               e2 || n2
-                         --------------------                         (E_AMult)
-                         AMult e1 e2 || n1*n2
-]]
-*)
-
 End AExp.
 
 (* ####################################################### *)
-(* * Expressions With Variables *)
+(** ** Computational vs. Relational Definitions *)
+
+(** For the definitions of evaluation for arithmetic and boolean
+    expressions, the choice of whether to use functional or relational
+    definitions is mainly a matter of taste.  In general, Coq has
+    somewhat better support for working with relations.  On the other
+    hand, in some sense function definitions carry more information,
+    because functions are necessarily deterministic and defined on all
+    arguments; for a relation we have to show these properties
+    explicitly if we need them. Functions also take advantage of Coq's
+    computations mechanism.
+
+    However, there are circumstances where relational definitions of
+    evaluation are preferable to functional ones.  *)
+
+Module aevalR_division.
+
+(** For example, suppose that we wanted to extend the arithmetic
+    operations by considering also a division operation:*)
+
+Inductive aexp : Type :=
+  | ANum : nat -> aexp
+  | APlus : aexp -> aexp -> aexp
+  | AMinus : aexp -> aexp -> aexp
+  | AMult : aexp -> aexp -> aexp
+  | ADiv : aexp -> aexp -> aexp.   (* <--- new *)
+
+(** Extending the definition of [aeval] to handle this new operation
+    would not be straightforward (what should we return as the result
+    of [ADiv (ANum 5) (ANum 0)]?).  But extending [aevalR] is
+    straightforward. *)
+
+Inductive aevalR : aexp -> nat -> Prop :=
+  | E_ANum : forall (n:nat),
+      (ANum n) || n
+  | E_APlus : forall (a1 a2: aexp) (n1 n2 : nat),
+      (a1 || n1) -> (a2 || n2) -> (APlus a1 a2) || (n1 + n2)
+  | E_AMinus : forall (a1 a2: aexp) (n1 n2 : nat),
+      (a1 || n1) -> (a2 || n2) -> (AMinus a1 a2) || (n1 - n2)
+  | E_AMult :  forall (a1 a2: aexp) (n1 n2 : nat),
+      (a1 || n1) -> (a2 || n2) -> (AMult a1 a2) || (n1 * n2)
+  | E_ADiv :  forall (a1 a2: aexp) (n1 n2 n3: nat),
+      (a1 || n1) -> (a2 || n2) -> (mult n2 n3 = n1) -> (ADiv a1 a2) || n3
+
+where "a '||' n" := (aevalR a n) : type_scope.
+
+End aevalR_division.
+Module aevalR_extended.
+
+Inductive aexp : Type :=
+  | AAny  : aexp                   (* <--- NEW *)
+  | ANum : nat -> aexp
+  | APlus : aexp -> aexp -> aexp
+  | AMinus : aexp -> aexp -> aexp
+  | AMult : aexp -> aexp -> aexp.
+
+(** Again, extending [aeval] would be tricky (because evaluation is
+    _not_ a deterministic function from expressions to numbers), but
+    extending [aevalR] is no problem: *)
+
+Inductive aevalR : aexp -> nat -> Prop :=
+  | E_Any : forall (n:nat),
+      AAny || n                 (* <--- new *)
+  | E_ANum : forall (n:nat),
+      (ANum n) || n
+  | E_APlus : forall (a1 a2: aexp) (n1 n2 : nat),
+      (a1 || n1) -> (a2 || n2) -> (APlus a1 a2) || (n1 + n2)
+  | E_AMinus : forall (a1 a2: aexp) (n1 n2 : nat),
+      (a1 || n1) -> (a2 || n2) -> (AMinus a1 a2) || (n1 - n2)
+  | E_AMult :  forall (a1 a2: aexp) (n1 n2 : nat),
+      (a1 || n1) -> (a2 || n2) -> (AMult a1 a2) || (n1 * n2)
+
+where "a '||' n" := (aevalR a n) : type_scope.
+
+End aevalR_extended.
+
+(*  * Expressions With Variables *)
 (** * 変数を持つ式 *)
 
-(* Now let's turn our attention back to defining Imp.  The next thing
-    we need to do is to enrich our arithmetic and boolean expressions
+(** Let's turn our attention back to defining Imp.  The next thing we
+    need to do is to enrich our arithmetic and boolean expressions
     with variables.  To keep things simple, we'll assume that all
     variables are global and that they only hold numbers. *)
-(** さて、Impの定義に戻りましょう。次にしなければならないことは、
+(** Impの定義に戻ることにしましょう。次にしなければならないことは、
     算術式とブール式に変数を拡張することです。
     話を単純にするため、すべての変数はグローバルで、数値だけを持つとしましょう。 *)
 
 (* ##################################################### *)
-(* ** Identifiers *)
+(*  ** Identifiers *)
 (** ** 識別子 *)
 
-(* To begin, we'll need to formalize _identifiers_, such as program
-    variables.  We could use strings for this, or (in a real compiler)
-    some kind of fancier structures like pointers into a symbol table.
-    But for simplicity let's just use natural numbers as identifiers.
+(*  To begin, we'll need to formalize _identifiers_ such as program
+    variables.  We could use strings for this -- or, in a real
+    compiler, fancier structures like pointers into a symbol table.
+    But for simplicity let's just use natural numbers as identifiers. *)
 
-    (We hide this section in a module because these definitions are
-    actually in [SfLib.v], but we want to repeat them here so that we
+(*  (We hide this section in a module because these definitions are
+    actually in [SfLib], but we want to repeat them here so that we
     can explain them.) *)
 (** 始めに、プログラム変数などの識別子(_identifiers_)を形式化しなければなりません。
     このために文字列を使うこともできるでしょうし、(実際のコンパイラでは)
@@ -1171,91 +1224,61 @@ End AExp.
     (このセクションをモジュールに隠します。それは、これらの定義が実際には[SfLib_J.v]
     にあるからです。しかし説明のためにここで繰り返します。) *)
 
-Module Id.
+Module Id. 
 
-(* We define a new inductive datatype [Id] so that we won't confuse
-    identifiers and numbers. *)
-(** 新しいデータタイプ[Id]を定義して、識別子と数値を混乱しないようにします。 *)
+(*  We define a new inductive datatype [Id] so that we won't confuse
+    identifiers and numbers.  We use [sumbool] to define a computable
+    equality operator on [Id]. *)
+(** 新しいデータタイプ[Id]を定義して、識別子と数値を混乱しないようにします。 
+   [Id]についての計算可能な同値演算子を定義するために、[sumbool]を使用します。*)
 
 Inductive id : Type :=
   Id : nat -> id.
 
-Definition beq_id X1 X2 :=
-  match (X1, X2) with
-    (Id n1, Id n2) => beq_nat n1 n2
-  end.
-
-(* Now, having "wrapped" numbers as identifiers in this way, it
-    is convenient to recapitulate a few properties of numbers as
-    analogous properties of identifiers, so that we can work with
-    identifiers in definitions and proofs abstractly, without
-    unwrapping them to expose the underlying numbers.  Since all we
-    need to know about identifiers is whether they are the same or
-    different, just a few basic facts are all we need. *)
-(** さて、この方法で「覆った」数値を識別子としたので、
-    数値のいくつかの性質を、対応する識別子の性質として繰り返しておくのが便利です。
-    そうすると、定義や証明の中の識別子を、
-    覆いを開いて中の数値を晒すことなく抽象的に扱うことができます。
-    識別子について知らなければならないことは、識別子同士が同じか違うかだけなので、
-    本当に2、3のことだけが必要です。 *)
-
-Theorem beq_id_refl : forall X,
-  true = beq_id X X.
+Theorem eq_id_dec : forall id1 id2 : id, {id1 = id2} + {id1 <> id2}.
 Proof.
-  intros. destruct X.
-  apply beq_nat_refl.  Qed.
+   intros id1 id2.
+   destruct id1 as [n1]. destruct id2 as [n2].
+   destruct (eq_nat_dec n1 n2) as [Heq | Hneq].
+   Case "n1 = n2".
+     left. rewrite Heq. reflexivity.
+   Case "n1 <> n2".
+     right. intros contra. inversion contra. apply Hneq. apply H0.
+Defined. 
 
-(* **** Exercise: 1 star, optional (beq_id_eq) *)
-(** **** 練習問題: ★, optional (beq_id_eq) *)
-(* For this and the following exercises, do not use induction, but
-    rather apply similar results already proved for natural numbers.
-    Some of the tactics mentioned above may prove useful. *)
-(** この問題とそれに続く練習問題では、帰納法を使わずに、
-    既に証明した自然数の同様の結果を適用しなさい。
-    上述したいくつかのタクティックが使えるかもしれません。 *)
+(* The following lemmas will be useful for rewriting terms involving [eq_id_dec]. *)
+(** 次の補題は、[eq_id_dec]を含む式を書き直すのに役立ちます。 *)
 
-Theorem beq_id_eq : forall i1 i2,
-  true = beq_id i1 i2 -> i1 = i2.
+Lemma eq_id : forall (T:Type) x (p q:T), 
+              (if eq_id_dec x x then p else q) = p. 
+Proof.
+  intros. 
+  destruct (eq_id_dec x x). 
+  Case "x = x". 
+    reflexivity.
+  Case "x <> x (impossible)". 
+    apply ex_falso_quodlibet; apply n; reflexivity. Qed.
+
+(** **** Exercise: 1 star, optional (neq_id) *)
+Lemma neq_id : forall (T:Type) x y (p q:T), x <> y -> 
+               (if eq_id_dec x y then p else q) = q. 
 Proof.
   (* FILL IN HERE *) Admitted.
 (** [] *)
 
-(* **** Exercise: 1 star, optional (beq_id_false_not_eq) *)
-(** **** 練習問題: ★, optional (beq_id_false_not_eq) *)
-Theorem beq_id_false_not_eq : forall i1 i2,
-  beq_id i1 i2 = false -> i1 <> i2.
-Proof.
-  (* FILL IN HERE *) Admitted.
-(** [] *)
 
-(* **** Exercise: 1 star, optional (not_eq_beq_id_false) *)
-(** **** 練習問題: ★, optional (not_eq_beq_id_false) *)
-Theorem not_eq_beq_id_false : forall i1 i2,
-  i1 <> i2 -> beq_id i1 i2 = false.
-Proof.
-  (* FILL IN HERE *) Admitted.
-(** [] *)
-
-(* **** Exercise: 1 star, optional (beq_id_sym) *)
-(** **** 練習問題: ★, optional (beq_id_sym) *)
-Theorem beq_id_sym: forall i1 i2,
-  beq_id i1 i2 = beq_id i2 i1.
-Proof.
-  (* FILL IN HERE *) Admitted.
-(** [] *)
-
-End Id.
+End Id. 
 
 (* ####################################################### *)
-(* ** States *)
+(*  ** States *)
 (** ** 状態 *)
 
-(* A _state_ represents the current values of all the variables at
+(** A _state_ represents the current values of all the variables at
     some point in the execution of a program. *)
 (** 状態(_state_)はプログラムの実行のある時点のすべての変数の現在値を表します。 *)
-(* For simplicity (to avoid dealing with partial functions), we
+(** For simplicity (to avoid dealing with partial functions), we
     let the state be defined for _all_ variables, even though any
-    given program is only going tomention a finite number of them. *)
+    given program is only going to mention a finite number of them. *)
 (** 簡単にするため(部分関数を扱うのを避けるため)、
     どのようなプログラムも有限個の変数しか使わないにもかかわらず、
     状態はすべての変数について値を定義しているものとします。 *)
@@ -1265,32 +1288,33 @@ Definition state := id -> nat.
 Definition empty_state : state :=
   fun _ => 0.
 
-Definition update (st : state) (X:id) (n : nat) : state :=
-  fun X' => if beq_id X X' then n else st X'.
+Definition update (st : state) (x : id) (n : nat) : state :=
+  fun x' => if eq_id_dec x x' then n else st x'.
 
-(* We'll need a few simple properties of [update]. *)
-(** [update]についての単純な性質が必要です。 *)
+(** For proofs involving states, we'll need several simple properties
+    of [update]. *)
+(** 状態を含む証明のために、[update]についての単純な性質が必要です。 *)
 
-(* **** Exercise: 2 stars, optional (update_eq) *)
-(** **** 練習問題: ★★, optional (update_eq) *)
-Theorem update_eq : forall n X st,
-  (update st X n) X = n.
+(*  **** Exercise: 1 star (update_eq) *)
+(** **** 練習問題: ★, optional (update_eq) *)
+Theorem update_eq : forall n x st,
+  (update st x n) x = n.
 Proof.
   (* FILL IN HERE *) Admitted.
 (** [] *)
 
-(* **** Exercise: 2 stars, optional (update_neq) *)
-(** **** 練習問題: ★★, optional (update_neq) *)
-Theorem update_neq : forall V2 V1 n st,
-  beq_id V2 V1 = false ->
-  (update st V2 n) V1 = (st V1).
+(*  **** Exercise: 1 star (update_neq) *)
+(** **** 練習問題: ★, optional (update_neq) *)
+Theorem update_neq : forall x2 x1 n st,
+  x2 <> x1 ->                        
+  (update st x2 n) x1 = (st x1).
 Proof.
   (* FILL IN HERE *) Admitted.
 (** [] *)
 
-(* **** Exercise: 2 stars, optional (update_example) *)
-(** **** 練習問題: ★★, optional (update_example) *)
-(* Before starting to play with tactics, make sure you understand
+(*  **** Exercise: 1 star (update_example) *)
+(** **** 練習問題: ★, optional (update_example) *)
+(** Before starting to play with tactics, make sure you understand
     exactly what the theorem is saying! *)
 (** タクティックを使って遊び始める前に、
     定理が言っていることを正確に理解していることを確認しなさい! *)
@@ -1301,39 +1325,37 @@ Proof.
   (* FILL IN HERE *) Admitted.
 (** [] *)
 
-(* **** Exercise: 2 stars (update_shadow) *)
-(** **** 練習問題: ★★ (update_shadow) *)
-Theorem update_shadow : forall x1 x2 k1 k2 (f : state),
-   (update  (update f k2 x1) k2 x2) k1 = (update f k2 x2) k1.
+(** **** Exercise: 1 star (update_shadow) *)
+Theorem update_shadow : forall n1 n2 x1 x2 (st : state),
+   (update  (update st x2 n1) x2 n2) x1 = (update st x2 n2) x1.
 Proof.
   (* FILL IN HERE *) Admitted.
 (** [] *)
 
-(* **** Exercise: 2 stars, optional (update_same) *)
-(** **** 練習問題: ★★, optional (update_same) *)
-Theorem update_same : forall x1 k1 k2 (f : state),
-  f k1 = x1 ->
-  (update f k1 x1) k2 = f k2.
+(** **** Exercise: 2 stars (update_same) *)
+Theorem update_same : forall n1 x1 x2 (st : state),
+  st x1 = n1 ->
+  (update st x1 n1) x2 = st x2.
 Proof.
   (* FILL IN HERE *) Admitted.
 (** [] *)
 
-(* **** Exercise: 2 stars, optional (update_permute) *)
-(** **** 練習問題: ★★, optional (update_permute) *)
-Theorem update_permute : forall x1 x2 k1 k2 k3 f,
-  beq_id k2 k1 = false ->
-  (update (update f k2 x1) k1 x2) k3 = (update (update f k1 x2) k2 x1) k3.
+(** **** Exercise: 3 stars (update_permute) *)
+Theorem update_permute : forall n1 n2 x1 x2 x3 st,
+  x2 <> x1 -> 
+  (update (update st x2 n1) x1 n2) x3 = (update (update st x1 n2) x2 n1) x3.
 Proof.
   (* FILL IN HERE *) Admitted.
 (** [] *)
 
 (* ################################################### *)
-(* ** Syntax  *)
+(*  ** Syntax  *)
 (** ** 構文  *)
 
-(* We can add variables to the arithmetic expressions we had before by
+(*  We can add variables to the arithmetic expressions we had before by
     simply adding one more constructor: *)
 (** 前に定義した算術式に、単にもう1つコンストラクタを追加することで変数を追加できます: *)
+
 
 Inductive aexp : Type :=
   | ANum : nat -> aexp
@@ -1347,14 +1369,14 @@ Tactic Notation "aexp_cases" tactic(first) ident(c) :=
   [ Case_aux c "ANum" | Case_aux c "AId" | Case_aux c "APlus"
   | Case_aux c "AMinus" | Case_aux c "AMult" ].
 
-(* Shorthands for variables: *)
-(** 変数の略記法: *)
-
+(** Defining a few variable names as notational shorthands will make
+    examples easier to read: *)
+(** 読み易い例を作りやすくするため、幾つかの変数名を定義しておきましょう *)
 Definition X : id := Id 0.
 Definition Y : id := Id 1.
 Definition Z : id := Id 2.
 
-(* (This convention for naming program variables ([X], [Y],
+(** (This convention for naming program variables ([X], [Y],
     [Z]) clashes a bit with our earlier use of uppercase letters for
     types.  Since we're not using polymorphism heavily in this part of
     the course, this overloading should not cause confusion.) *)
@@ -1362,7 +1384,7 @@ Definition Z : id := Id 2.
     型に大文字の記号を使うという以前の使用法と衝突します。
     コースのこの部分では多相性を多用はしないので、このことが混乱を招くことはないはずです。) *)
 
-(* The definition of [bexp]s is the same as before (using the new
+(** The definition of [bexp]s is the same as before (using the new
     [aexp]s): *)
 (** [bexp]の定義は前と同じです(ただし新しい[aexp]を使います): *)
 
@@ -1380,24 +1402,24 @@ Tactic Notation "bexp_cases" tactic(first) ident(c) :=
   | Case_aux c "BLe" | Case_aux c "BNot" | Case_aux c "BAnd" ].
 
 (* ################################################### *)
-(* ** Evaluation  *)
+(*  ** Evaluation  *)
 (** ** 評価  *)
 
-(* The arith and boolean evaluators are extended to handle
+(** The arith and boolean evaluators can be extended to handle
     variables in the obvious way: *)
 (** 算術とブールの評価器は、自明な方法で変数を扱うように拡張されます: *)
 
-Fixpoint aeval (st : state) (e : aexp) : nat :=
-  match e with
+Fixpoint aeval (st : state) (a : aexp) : nat :=
+  match a with
   | ANum n => n
-  | AId X => st X                                        (* <----- NEW *)
+  | AId x => st x                                        (* <----- NEW *)
   | APlus a1 a2 => (aeval st a1) + (aeval st a2)
   | AMinus a1 a2  => (aeval st a1) - (aeval st a2)
   | AMult a1 a2 => (aeval st a1) * (aeval st a2)
   end.
 
-Fixpoint beval (st : state) (e : bexp) : bool :=
-  match e with
+Fixpoint beval (st : state) (b : bexp) : bool :=
+  match b with
   | BTrue       => true
   | BFalse      => false
   | BEq a1 a2   => beq_nat (aeval st a1) (aeval st a2)
@@ -1419,56 +1441,48 @@ Example bexp1 :
 Proof. reflexivity. Qed.
 
 (* ####################################################### *)
-(* * Commands *)
+(*  * Commands *)
 (** * コマンド *)
 
 (*  Now we are ready define the syntax and behavior of Imp
-    _commands_ (or _statements_). *)
+    _commands_ (often called _statements_). *)
 (** さて、Imp コマンド (または主張) の構文と挙動を定義する準備が出来ました *)
 
 (* ################################################### *)
 (*  ** Syntax *)
 (** ** 構文 *)
 
-(*  Informally, commands are described by the following BNF
+(** Informally, commands [c] are described by the following BNF
     grammar:
-[[
-     com ::= 'SKIP'
-           | X '::=' aexp
-           | com ';' com
-           | 'WHILE' bexp 'DO' com 'END'
-           | 'IFB' bexp 'THEN' com 'ELSE' com 'FI'
-]]
+     c ::= SKIP
+         | x ::= a
+         | c ; c
+         | WHILE b DO c END
+         | IFB b THEN c ELSE c FI
     For example, here's the factorial function in Imp.
-[[
      Z ::= X;
      Y ::= 1;
      WHILE not (Z = 0) DO
        Y ::= Y * Z;
        Z ::= Z - 1
      END
-]]
    When this command terminates, the variable [Y] will contain the
-   factorial of the variable [X].
+   factorial of the initial value of [X].
 *)
 (** 非形式的には、コマンドは以下の BNF で表現されます。
     構文:
-[[
      com ::= 'SKIP'
            | X '::=' aexp
            | com ';' com
            | 'WHILE' bexp 'DO' com 'END'
            | 'IFB' bexp 'THEN' com 'ELSE' com 'FI'
-]]
     例えば、Imp における階乗関数は以下のようになります。
-[[
      Z ::= X;
      Y ::= 1;
      WHILE not (Z = 0) DO
        Y ::= Y * Z;
        Z ::= Z - 1
      END
-]]
    このコマンドが終わったとき、変数 [Y] は変数 [X] の階乗の値を持つでしょう。
 *)
 
@@ -1484,17 +1498,16 @@ Inductive com : Type :=
 
 Tactic Notation "com_cases" tactic(first) ident(c) :=
   first;
-  [ Case_aux c "SKIP" | Case_aux c "::=" | Case_aux c ";"
+  [ Case_aux c "SKIP" | Case_aux c "::=" | Case_aux c ";;"
   | Case_aux c "IFB" | Case_aux c "WHILE" ].
 
 (*  As usual, we can use a few [Notation] declarations to make things
-    more readable.  However, we need to be a bit careful to avoid
-    conflicts with Coq's built-in notations, so we'll keep this
-    light -- in particular, we won't introduce any notations for
-    [aexps] and [bexps] to avoid confusion with the numerical and
-    boolean operators we've already defined.  (We use the keyword
-    [IFB] for conditionals instead of the usual [IF] for similar
-    reasons.) *)
+    more readable.  We need to be a bit careful to avoid conflicts
+    with Coq's built-in notations, so we'll keep this light -- in
+    particular, we won't introduce any notations for [aexps] and
+    [bexps] to avoid confusion with the numerical and boolean
+    operators we've already defined.  We use the keyword [IFB] for
+    conditionals instead of [IF], for similar reasons. *)
 (** いつものとおり、より読みやすいよう、いくつかの [Notation] 宣言が使えます。
     しかし、Coq の組み込みの表記と衝突しないよう、少し気をつける必要があります 
     (手軽さを維持しつつ！)。
@@ -1506,14 +1519,14 @@ Tactic Notation "com_cases" tactic(first) ident(c) :=
 
 Notation "'SKIP'" :=
   CSkip.
-Notation "X '::=' a" :=
-  (CAss X a) (at level 60).
-Notation "c1 ; c2" :=
+Notation "x '::=' a" :=
+  (CAss x a) (at level 60).
+Notation "c1 ;; c2" :=
   (CSeq c1 c2) (at level 80, right associativity).
 Notation "'WHILE' b 'DO' c 'END'" :=
   (CWhile b c) (at level 80, right associativity).
-Notation "'IFB' e1 'THEN' e2 'ELSE' e3 'FI'" :=
-  (CIf e1 e2 e3) (at level 80, right associativity).
+Notation "'IFB' c1 'THEN' c2 'ELSE' c3 'FI'" :=
+  (CIf c1 c2 c3) (at level 80, right associativity).
 
 (*  For example, here is the factorial function again, written as a
     formal definition to Coq: *)
@@ -1521,19 +1534,16 @@ Notation "'IFB' e1 'THEN' e2 'ELSE' e3 'FI'" :=
     以下のようになります。*)
 
 Definition fact_in_coq : com :=
-  Z ::= AId X;
-  Y ::= ANum 1;
+  Z ::= AId X;;
+  Y ::= ANum 1;;
   WHILE BNot (BEq (AId Z) (ANum 0)) DO
-    Y ::= AMult (AId Y) (AId Z);
+    Y ::= AMult (AId Y) (AId Z);;
     Z ::= AMinus (AId Z) (ANum 1)
   END.
 
 (* ####################################################### *)
 (*  ** Examples *)
 (** ** 例 *)
-
-(*  Here are some more examples... *)
-(** 以下に、さらなる例を挙げます。 *)
 
 (*  Assignment: *)
 (** 割り当て: *)
@@ -1545,7 +1555,7 @@ Definition XtimesYinZ : com :=
   Z ::= (AMult (AId X) (AId Y)).
 
 Definition subtract_slowly_body : com :=
-  Z ::= AMinus (AId Z) (ANum 1) ;
+  Z ::= AMinus (AId Z) (ANum 1) ;;
   X ::= AMinus (AId X) (ANum 1).
 
 (*  Loops: *)
@@ -1557,8 +1567,8 @@ Definition subtract_slowly : com :=
   END.
 
 Definition subtract_3_from_5_slowly : com :=
-  X ::= ANum 3 ;
-  Z ::= ANum 5 ;
+  X ::= ANum 3 ;;
+  Z ::= ANum 5 ;;
   subtract_slowly.
 
 (*  An infinite loop: *)
@@ -1569,262 +1579,105 @@ Definition loop : com :=
     SKIP
   END.
 
-(*  Factorial again (broken up into smaller pieces this time, for
-    convenience when we come back to proving things about it
-    later).  *)
-(** 階乗関数再び (あとで戻って証明するとき便利なように、
-    細かい部品に分割してあります)。 *)
-
-Definition fact_body : com :=
-  Y ::= AMult (AId Y) (AId Z) ;
-  Z ::= AMinus (AId Z) (ANum 1).
-
-Definition fact_loop : com :=
-  WHILE BNot (BEq (AId Z) (ANum 0)) DO
-    fact_body
-  END.
-
-Definition fact_com : com :=
-  Z ::= AId X ;
-  Y ::= ANum 1 ;
-  fact_loop.
-
 (* ################################################################ *)
 (*  * Evaluation *)
-(** * 評価 *)
+(** ** 評価  *)
 
-(* Next we need to define what it means to evaluate an Imp command.
-    [WHILE] loops actually make this a bit tricky... *)
+(** Next we need to define what it means to evaluate an Imp command.
+    The fact that [WHILE] loops don't necessarily terminate makes defining
+    an evaluation function tricky... *)
 (** 次に、Imp のコマンドの実行が何を意味するかを定義する必要があります。
-    [WHILE] ループは、これを少々扱いにくいものにしています ... *)
+    [WHILE] ループは、必ずしも終了しないという事実が、これを少々扱いにくいものにしています ... *)
 
 (* #################################### *)
-(*  ** Evaluation Function *)
-(** ** 評価関数 *)
+(*  ** Evaluation as a Function (Failed Attempt) *)
+(** ** 評価関数(失敗バージョン) *)
 
-(*  Here's a first try at an evaluation function for commands,
-    omitting [WHILE]. *)
+(*  Here's an attempt at defining an evaluation function for commands,
+    omitting the [WHILE] case. *)
 (** 以下は [WHILE] 以外のコマンドの評価関数を得ようとした、最初の試みです。 *)
 
-Fixpoint ceval_step1 (st : state) (c : com) : state :=
+Fixpoint ceval_fun_no_while (st : state) (c : com) : state :=
   match c with
     | SKIP =>
         st
-    | l ::= a1 =>
-        update st l (aeval st a1)
-    | c1 ; c2 =>
-        let st' := ceval_step1 st c1 in
-        ceval_step1 st' c2
+    | x ::= a1 =>
+        update st x (aeval st a1)
+    | c1 ;; c2 =>
+        let st' := ceval_fun_no_while st c1 in
+        ceval_fun_no_while st' c2
     | IFB b THEN c1 ELSE c2 FI =>
         if (beval st b)
-          then ceval_step1 st c1
-          else ceval_step1 st c2
-    | WHILE b1 DO c1 END =>
+          then ceval_fun_no_while st c1
+          else ceval_fun_no_while st c2
+    | WHILE b DO c END =>
         st  (* bogus *)
   end.
 
-(*  Second try, using an extra numeric argument as a "step index" to
-    ensure that evaluation always terminates. *)
-(** 次の試みでは、評価が常に停止することを保証するため、
-    数の引数を追加して「ステップ指数」として用いています。*)
-
-Fixpoint ceval_step2 (st : state) (c : com) (i : nat) : state :=
-  match i with
-  | O => empty_state
-  | S i' =>
+(** In a traditional functional programming language like ML or
+    Haskell we could write the [WHILE] case as follows:
+<<
+  Fixpoint ceval_fun (st : state) (c : com) : state :=
     match c with
-      | SKIP =>
-          st
-      | l ::= a1 =>
-          update st l (aeval st a1)
-      | c1 ; c2 =>
-          let st' := ceval_step2 st c1 i' in
-          ceval_step2 st' c2 i'
-      | IFB b THEN c1 ELSE c2 FI =>
-          if (beval st b)
-            then ceval_step2 st c1 i'
-            else ceval_step2 st c2 i'
-      | WHILE b1 DO c1 END =>
+      ...
+      | WHILE b DO c END =>
           if (beval st b1)
-          then let st' := ceval_step2 st c1 i' in
-               ceval_step2 st' c i'
-          else st
-    end
-  end.
+            then ceval_fun st (c1; WHILE b DO c END)
+            else st
+    end.
+>>
+    Coq doesn't accept such a definition ("Error: Cannot guess
+    decreasing argument of fix") because the function we want to
+    define is not guaranteed to terminate. Indeed, it doesn't always
+    terminate: for example, the full version of the [ceval_fun]
+    function applied to the [loop] program above would never
+    terminate. Since Coq is not just a functional programming
+    language, but also a consistent logic, any potentially
+    non-terminating function needs to be rejected. Here is
+    an (invalid!) Coq program showing what would go wrong if Coq
+    allowed non-terminating recursive functions:
+<<
+     Fixpoint loop_false (n : nat) : False := loop_false n.
+>>
+    That is, propositions like [False] would become provable
+    (e.g. [loop_false 0] would be a proof of [False]), which
+    would be a disaster for Coq's logical consistency.
 
-(*  _Note_: It is tempting to think that the index [i] here is
-    counting the "number of steps of evaluation."  But if you look
-    closely you'll see that this is not the case: for example, in the
-    rule for sequencing, the same [i] is passed to both recursive
-    calls.  Understanding the exact way that [i] is treated will be
-    important in the proof of [ceval__ceval_step], which is given as
-    an exercise below. *)
-(** 注: ここでの指数 [i] は「評価のステップ数」を数えるものだろうか？
-    という点が気になります。しかしよく見ると、そうではないと分かります。
-    例えば、直列実行に対する規則では、2 つの再帰呼び出しに同じ [i] が渡されています。
-    [i] がどのように扱われているのかを正確に理解することは、
-    以下で演習問題として与えられている [ceval__ceval_step] の証明で重要となるでしょう。 *)
-
-(*  Third try, returning an [option state] instead of just a [state]
-    so that we can distinguish between normal and abnormal
-    termination. *)
-(** 3 つ目の試みでは、単なる [state] の代わりに [option state] を返すようにしています。
-    こうすると、通常終了と異常終了を区別出来ます。*)
-
-Fixpoint ceval_step3 (st : state) (c : com) (i : nat)
-                    : option state :=
-  match i with
-  | O => None
-  | S i' =>
-    match c with
-      | SKIP =>
-          Some st
-      | l ::= a1 =>
-          Some (update st l (aeval st a1))
-      | c1 ; c2 =>
-          match (ceval_step3 st c1 i') with
-          | Some st' => ceval_step3 st' c2 i'
-          | None => None
-          end
-      | IFB b THEN c1 ELSE c2 FI =>
-          if (beval st b)
-            then ceval_step3 st c1 i'
-            else ceval_step3 st c2 i'
-      | WHILE b1 DO c1 END =>
-          if (beval st b1)
-          then match (ceval_step3 st c1 i') with
-               | Some st' => ceval_step3 st' c i'
-               | None => None
-               end
-          else Some st
-    end
-  end.
-
-(*  We can improve the readability of this definition by introducing a
-    bit of auxiliary notation to hide the "plumbing" involved in
-    repeatedly matching against optional states. *)
-(** オプション状態に対する場合分けに繰り返し含まれている「配管」を隠すための、
-    補助的なちょっとした記法を導入すると、この定義の読みやすさは改善出来ます。*)
-
-Notation "'LETOPT' x <== e1 'IN' e2"
-   := (match e1 with
-         | Some x => e2
-         | None => None
-       end)
-   (right associativity, at level 60).
-
-Fixpoint ceval_step (st : state) (c : com) (i : nat)
-                    : option state :=
-  match i with
-  | O => None
-  | S i' =>
-    match c with
-      | SKIP =>
-          Some st
-      | l ::= a1 =>
-          Some (update st l (aeval st a1))
-      | c1 ; c2 =>
-          LETOPT st' <== ceval_step st c1 i' IN
-          ceval_step st' c2 i'
-      | IFB b THEN c1 ELSE c2 FI =>
-          if (beval st b)
-            then ceval_step st c1 i'
-            else ceval_step st c2 i'
-      | WHILE b1 DO c1 END =>
-          if (beval st b1)
-          then LETOPT st' <== ceval_step st c1 i' IN
-               ceval_step st' c i'
-          else Some st
-    end
-  end.
-
-Definition test_ceval (st:state) (c:com) :=
-  match ceval_step st c 500 with
-  | None    => None
-  | Some st => Some (st X, st Y, st Z)
-  end.
-
-(*
-Eval compute in
-  (test_ceval empty_state
-      (X ::= ANum 2;
-       IFB BLe (AId X) (ANum 1)
-         THEN Y ::= ANum 3
-         ELSE Z ::= ANum 4
-       FI)).
-====>
-   Some (2, 0, 4)
-*)
-
-(* **** Exercise: 2 stars, recommended (pup_to_n) *)
-(** **** 練習問題: ★★, recommended (pup_to_n) *)
-(*  Write an Imp program that sums the numbers from [1] to
-   [X] (inclusive: [1 + 2 + ... + X]) in the variable [Y].  Make sure
-   your solution satisfies the test that follows. *)
-(** [1] から [X] までの整数を変数 [Y] に足す (つまり [1 + 2 + ... + X]) 
-    Imp プログラムを書きなさい。下に示したテストを満たすことを確認しなさい。 *)
-
-Definition pup_to_n : com :=
-  (* FILL IN HERE *) admit.
-
-(*
-Example pup_to_n_1 :
-  test_ceval (update empty_state X 5) pup_to_n
-  = Some (0, 15, 0).
-Proof. reflexivity. Qed.
-*)
-(** [] *)
-
-(*  **** Exercise: 2 stars, optional (peven) *)
-(** **** 練習問題: ★★, optional (peven) *)
-(*  Write a [While] program that sets [Z] to [0] if [X] is even and
-    sets [Z] to [1] otherwise.  Use [ceval_test] to test your
-    program. *)
-(** [X] が偶数だったら [Z] に [0] を、そうでなければ [Z] に [1] をセットする 
-    [While] プログラムを書きなさい。テストには [ceval_test] を使いなさい。 *)
-
-(* FILL IN HERE *)
-(** [] *)
+    Thus, because it doesn't terminate on all inputs, the full version
+    of [ceval_fun] cannot be written in Coq -- at least not without
+    additional tricks (see chapter [ImpCEvalFun] if curious). *)
 
 (* #################################### *)
 (*  ** Evaluation as a Relation *)
-(** ** 関係としての評価 *)
+(** * 関係としての評価 *)
 
-(*  Here's a better way: define [ceval] as a _relation_ rather than a
-    _function_ -- i.e., define it in [Prop] instead of [Type], as we
-    did for [aevalR] and [bevalR] above.
+(** Here's a better way: we define [ceval] as a _relation_ rather than
+    a _function_ -- i.e., we define it in [Prop] instead of [Type], as
+    we did for [aevalR] above. *)
 
-    This is an important change.  Besides freeing us from the
-    silliness of passing around step indices all over the place, it
-    gives us a lot more flexibility in the definition.  For example,
-    if we added concurrency features to the language, we'd want the
-    definition of evaluation to be non-deterministic -- i.e., not only
-    would it not be total, it would not even be a partial function! *)
-(** ここに改善策があります: [ceval] を関数ではなく関係 (_relation_) として定義しましょう。
-    つまり、上の [aevalR] と [bevalR] と同様に [Type] ではなく [Prop] で定義しましょう。
+(** This is an important change.  Besides freeing us from the awkward
+    workarounds that would be needed to define evaluation as a
+    function, it gives us a lot more flexibility in the definition.
+    For example, if we added concurrency features to the language,
+    we'd want the definition of evaluation to be non-deterministic --
+    i.e., not only would it not be total, it would not even be a
+    partial function! *)
 
-    これは重要な変更です。
-    ステップ指数をすべての場所で引き回す馬鹿馬鹿しさから解放してくれるのに加え、
-    定義での柔軟性を与えてくれます。
-    例えば、もし言語に並行性の要素を導入したら、評価の定義を非決定的に書きたくなるでしょう。
-    つまり、その関数は全関数でないだけでなく、部分関数ですらないかも知れません！*)
-
-(*  We'll use the notation [c / st || st'] for our [ceval] relation,
-    that is [c / st || st'] means that executing program [c] in a
-    starting state [st] results in an ending state [st'].  This can be
+(** We'll use the notation [c / st || st'] for our [ceval] relation:
+    [c / st || st'] means that executing program [c] in a starting
+    state [st] results in an ending state [st'].  This can be
     pronounced "[c] takes state [st] to [st']".
-[[[
                            ----------------                            (E_Skip)
                            SKIP / st || st
 
                            aeval st a1 = n
                    --------------------------------                     (E_Ass)
-                   l := a1 / st || (update st l n)
+                   x := a1 / st || (update st x n)
 
                            c1 / st || st'
                           c2 / st' || st''
                          -------------------                            (E_Seq)
-                         c1;c2 / st || st''
+                         c1;;c2 / st || st''
 
                           beval st b1 = true
                            c1 / st || st'
@@ -1838,88 +1691,46 @@ Proof. reflexivity. Qed.
 
                          beval st b1 = false
                     ------------------------------                 (E_WhileEnd)
-                    WHILE b1 DO c1 END / st || st
+                    WHILE b DO c END / st || st
 
                           beval st b1 = true
-                           c1 / st || st'
-                  WHILE b1 DO c1 END / st' || st''
+                           c / st || st'
+                  WHILE b DO c END / st' || st''
                   ---------------------------------               (E_WhileLoop)
-                    WHILE b1 DO c1 END / st || st''
-]]]
-*)
-(** [ceavl] 関係に対する表記として [c / st || st'] を使います。
-    正確に言うと、[c / st || st'] と書いたらプログラム [c] を初期状態 [st] で評価すると、
-    その結果は最終状態 [st'] になる、ということを意味します。
-    これは「[c] は状態 [st] を [st'] に持っていく」とも言えます。
-[[
-                           ----------------                            (E_Skip)
-                           SKIP / st || st
-
-                           aeval st a1 = n
-                   --------------------------------                     (E_Ass)
-                   l := a1 / st || (update st l n)
-
-                           c1 / st || st'
-                          c2 / st' || st''
-                         -------------------                            (E_Seq)
-                         c1;c2 / st || st''
-
-                          beval st b1 = true
-                           c1 / st || st'
-                -------------------------------------                (E_IfTrue)
-                IF b1 THEN c1 ELSE c2 FI / st || st'
-
-                         beval st b1 = false
-                           c2 / st || st'
-                -------------------------------------               (E_IfFalse)
-                IF b1 THEN c1 ELSE c2 FI / st || st'
-
-                         beval st b1 = false
-                    ------------------------------                 (E_WhileEnd)
-                    WHILE b1 DO c1 END / st || st
-
-                          beval st b1 = true
-                           c1 / st || st'
-                  WHILE b1 DO c1 END / st' || st''
-                  ---------------------------------               (E_WhileLoop)
-                    WHILE b1 DO c1 END / st || st''
-]]
+                    WHILE b DO c END / st || st''
 *)
 
-
-(*  Here is the formal definition.  (Make sure you understand
+(** Here is the formal definition.  (Make sure you understand
     how it corresponds to the inference rules.) *)
-(** 以下に形式的な定義を挙げます。
-    (上の推論規則とどのように対応するか、確認しておきましょう。) *)
 
 Reserved Notation "c1 '/' st '||' st'" (at level 40, st at level 39).
 
 Inductive ceval : com -> state -> state -> Prop :=
   | E_Skip : forall st,
       SKIP / st || st
-  | E_Ass  : forall st a1 n l,
+  | E_Ass  : forall st a1 n x,
       aeval st a1 = n ->
-      (l ::= a1) / st || (update st l n)
+      (x ::= a1) / st || (update st x n)
   | E_Seq : forall c1 c2 st st' st'',
       c1 / st  || st' ->
       c2 / st' || st'' ->
-      (c1 ; c2) / st || st''
-  | E_IfTrue : forall st st' b1 c1 c2,
-      beval st b1 = true ->
+      (c1 ;; c2) / st || st''
+  | E_IfTrue : forall st st' b c1 c2,
+      beval st b = true ->
       c1 / st || st' ->
-      (IFB b1 THEN c1 ELSE c2 FI) / st || st'
-  | E_IfFalse : forall st st' b1 c1 c2,
-      beval st b1 = false ->
+      (IFB b THEN c1 ELSE c2 FI) / st || st'
+  | E_IfFalse : forall st st' b c1 c2,
+      beval st b = false ->
       c2 / st || st' ->
-      (IFB b1 THEN c1 ELSE c2 FI) / st || st'
-  | E_WhileEnd : forall b1 st c1,
-      beval st b1 = false ->
-      (WHILE b1 DO c1 END) / st || st
-  | E_WhileLoop : forall st st' st'' b1 c1,
-      beval st b1 = true ->
-      c1 / st || st' ->
-      (WHILE b1 DO c1 END) / st' || st'' ->
-      (WHILE b1 DO c1 END) / st || st''
+      (IFB b THEN c1 ELSE c2 FI) / st || st'
+  | E_WhileEnd : forall b st c,
+      beval st b = false ->
+      (WHILE b DO c END) / st || st
+  | E_WhileLoop : forall st st' st'' b c,
+      beval st b = true ->
+      c / st || st' ->
+      (WHILE b DO c END) / st' || st'' ->
+      (WHILE b DO c END) / st || st''
 
   where "c1 '/' st '||' st'" := (ceval c1 st st').
 
@@ -1929,17 +1740,13 @@ Tactic Notation "ceval_cases" tactic(first) ident(c) :=
   | Case_aux c "E_IfTrue" | Case_aux c "E_IfFalse"
   | Case_aux c "E_WhileEnd" | Case_aux c "E_WhileLoop" ].
 
-(*  The cost of defining evaluation as a relation instead of a
+(** The cost of defining evaluation as a relation instead of a
     function is that we now need to construct _proofs_ that some
     program evaluates to some result state, rather than just letting
     Coq's computation mechanism do it for us. *)
-(** 評価を関数ではなく関係として定義することのコストは、
-    あるプログラムを実行した結果がとある状態になる、
-    というのを Coq の計算機構にやってもらうだけではなく、
-    その「証明」を構築する必要がある、ということです。*)
 
 Example ceval_example1:
-    (X ::= ANum 2;
+    (X ::= ANum 2;;
      IFB BLe (AId X) (ANum 1)
        THEN Y ::= ANum 3
        ELSE Z ::= ANum 4
@@ -1956,194 +1763,48 @@ Proof.
       reflexivity.
       apply E_Ass. reflexivity.  Qed.
 
-(*  **** Exercise: 2 stars (ceval_example2) *)
-(** **** 練習問題: ★★ (ceval_example2) *)
+(** **** Exercise: 2 stars (ceval_example2) *)
 Example ceval_example2:
-    (X ::= ANum 0; Y ::= ANum 1; Z ::= ANum 2) / empty_state ||
+    (X ::= ANum 0;; Y ::= ANum 1;; Z ::= ANum 2) / empty_state ||
     (update (update (update empty_state X 0) Y 1) Z 2).
 Proof.
   (* FILL IN HERE *) Admitted.
 (** [] *)
 
-(* ################################################################ *)
-(*  ** Equivalence of Relational and Step-Indexed Evaluation *)
-(** ** 関係による評価とステップ指数を利用した評価の等価性 *)
+(** **** Exercise: 3 stars, advanced (pup_to_n) *)
+(** Write an Imp program that sums the numbers from [1] to
+   [X] (inclusive: [1 + 2 + ... + X]) in the variable [Y].
+   Prove that this program executes as intended for X = 2
+   (this latter part is trickier than you might expect). *)
 
-(* As with arithmetic and boolean expressions, we'd hope that
-    the two alternative definitions of evaluation actually boil down
-    to the same thing.  This section shows that this is the case.
-    Make sure you understand the statements of the theorems and can
-    follow the structure of the proofs. *)
-(** 算術式とブール式で行ったように、2 つの評価の定義が本当に、
-    結局のところ同じものになるのかを確認したくなるでしょう。
-    この章では、それを確認します。定理の主張を理解して、
-    証明の構造を追えることを確認しておいて下さい。*)
+Definition pup_to_n : com :=
+  (* FILL IN HERE *) admit.
 
-Theorem ceval_step__ceval: forall c st st',
-      (exists i, ceval_step st c i = Some st') ->
-      c / st || st'.
+Theorem pup_to_2_ceval :
+  pup_to_n / (update empty_state X 2) ||
+    update (update (update (update (update (update empty_state
+      X 2) Y 0) Y 2) X 1) Y 3) X 0.
 Proof.
-  intros c st st' H.
-  inversion H as [i E].
-  clear H.
-  generalize dependent st'.
-  generalize dependent st.
-  generalize dependent c.
-  induction i as [| i' ].
-
-  Case "i = 0 -- contradictory".
-    intros c st st' H. inversion H.
-
-  Case "i = S i'".
-    intros c st st' H.
-    com_cases (destruct c) SCase;
-           simpl in H; inversion H; subst; clear H.
-      SCase "SKIP". apply E_Skip.
-      SCase "::=". apply E_Ass. reflexivity.
-
-      SCase ";".
-        remember (ceval_step st c1 i') as r1. destruct r1.
-        SSCase "Evaluation of r1 terminates normally".
-          apply E_Seq with s.
-            apply IHi'. rewrite Heqr1. reflexivity.
-            apply IHi'. simpl in H1. assumption.
-        SSCase "Otherwise -- contradiction".
-          inversion H1.
-
-      SCase "IFB".
-        remember (beval st b) as r. destruct r.
-        SSCase "r = true".
-          apply E_IfTrue. rewrite Heqr. reflexivity.
-          apply IHi'. assumption.
-        SSCase "r = false".
-          apply E_IfFalse. rewrite Heqr. reflexivity.
-          apply IHi'. assumption.
-
-      SCase "WHILE". remember (beval st b) as r. destruct r.
-        SSCase "r = true".
-          remember (ceval_step st c i') as r1. destruct r1.
-          SSSCase "r1 = Some s".
-            apply E_WhileLoop with s. rewrite Heqr. reflexivity.
-            apply IHi'. rewrite Heqr1. reflexivity.
-            apply IHi'. simpl in H1. assumption.
-          SSSCase "r1 = None".
-            inversion H1.
-        SSCase "r = false".
-          inversion H1.
-          apply E_WhileEnd.
-          rewrite Heqr. subst. reflexivity.  Qed.
-
-(*  **** Exercise: 4 stars (ceval_step__ceval_inf) *)
-(** **** 練習問題: ★★★★ (ceval_step__ceval_inf) *)
-(* Write an informal proof of [ceval_step__ceval], following the
-    usual template.  (The template for case analysis on an inductively
-    defined value should look the same as for induction, except that
-    there is no induction hypothesis.)  Make your proof communicate
-    the main ideas to a human reader; do not simply transcribe the
-    steps of the formal proof.
-
-(* FILL IN HERE *)
-[]
-*)
-(** いつものテンプレートにのっとって、
-    [ceval_step__ceval] の形式的でない証明を書きましょう。
-    (帰納的に定義された値の場合分けに対するテンプレートは、
-    帰納法の仮定がないこと以外は帰納法と同じ見た目になるはずです。) 
-    単に形式的な証明のステップを書き写すだけでなく、
-    人間の読者に主要な考えが伝わるようにしなさい。
-
-(* FILL IN HERE *)
-[]
-*)
-
-Theorem ceval_step_more: forall i1 i2 st st' c,
-  i1 <= i2 ->
-  ceval_step st c i1 = Some st' ->
-  ceval_step st c i2 = Some st'.
-Proof.
-induction i1 as [|i1']; intros i2 st st' c Hle Hceval.
-  Case "i1 = 0".
-    inversion Hceval.
-  Case "i1 = S i1'".
-    destruct i2 as [|i2']. inversion Hle.
-    assert (Hle': i1' <= i2') by omega.
-    com_cases (destruct c) SCase.
-    SCase "SKIP".
-      simpl in Hceval. inversion Hceval.
-      reflexivity.
-    SCase "::=".
-      simpl in Hceval. inversion Hceval.
-      reflexivity.
-    SCase ";".
-      simpl in Hceval. simpl.
-      remember (ceval_step st c1 i1') as st1'o.
-      destruct st1'o.
-      SSCase "st1'o = Some".
-        symmetry in Heqst1'o.
-        apply (IHi1' i2') in Heqst1'o; try assumption.
-        rewrite Heqst1'o. simpl. simpl in Hceval.
-        apply (IHi1' i2') in Hceval; try assumption.
-      SSCase "st1'o = None".
-        inversion Hceval.
-
-    SCase "IFB".
-      simpl in Hceval. simpl.
-      remember (beval st b) as bval.
-      destruct bval; apply (IHi1' i2') in Hceval; assumption.
-
-    SCase "WHILE".
-      simpl in Hceval. simpl.
-      destruct (beval st b); try assumption.
-      remember (ceval_step st c i1') as st1'o.
-      destruct st1'o.
-      SSCase "st1'o = Some".
-        symmetry in Heqst1'o.
-        apply (IHi1' i2') in Heqst1'o; try assumption.
-        rewrite -> Heqst1'o. simpl. simpl in Hceval.
-        apply (IHi1' i2') in Hceval; try assumption.
-      SSCase "i1'o = None".
-        simpl in Hceval. inversion Hceval.  Qed.
-
-(*  **** Exercise: 3 stars, recommended (ceval__ceval_step) *)
-(** **** 練習問題: ★★★, recommended (ceval__ceval_step) *)
-(*  Finish the following proof.  You'll need [ceval_step_more] in a
-    few places, as well as some basic facts about [<=] and [plus]. *)
-(** 以下の証明を完成させなさい。何度か [ceval_step_more] が必要となり、
-    さらに [<=] と [plus] に関するいくつかの基本的な事実が必要となるでしょう。*)
-
-Theorem ceval__ceval_step: forall c st st',
-      c / st || st' ->
-      exists i, ceval_step st c i = Some st'.
-Proof.
-  intros c st st' Hce.
-  ceval_cases (induction Hce) Case.
   (* FILL IN HERE *) Admitted.
 (** [] *)
 
-Theorem ceval_and_ceval_step_coincide: forall c st st',
-      c / st || st'
-  <-> exists i, ceval_step st c i = Some st'.
-Proof.
-  intros c st st'.
-  split. apply ceval__ceval_step. apply ceval_step__ceval.
-Qed.
 
 (* ####################################################### *)
-(*  ** Determinacy of Evaluation *)
-(** ** 実行の決定性 *)
+(** ** Determinism of Evaluation *)
+(** ** 実行の決定論 *)
 
-(*  Changing from a computational to a relational definition of
+(** Changing from a computational to a relational definition of
     evaluation is a good move because it allows us to escape from the
-    artificial requirement (imposed by Coq's restrictions on Fixpoint
-    definitions) that evaluation should be a total function.  But it
-    also raises a question: Is the second definition of evaluation
-    actually a partial function?  That is, is it possible that,
-    beginning from the same state [st], we could evaluate some command
-    [c] in different ways to reach two different output states [st']
-    and [st'']?
+    artificial requirement (imposed by Coq's restrictions on
+    [Fixpoint] definitions) that evaluation should be a total
+    function.  But it also raises a question: Is the second definition
+    of evaluation actually a partial function?  That is, is it
+    possible that, beginning from the same state [st], we could
+    evaluate some command [c] in different ways to reach two different
+    output states [st'] and [st'']?
 
-    In fact, this cannot happen: the evaluation relation [ceval] is a
-    partial function.  Here's the proof: *)
+    In fact, this cannot happen: [ceval] is a partial function.
+    Here's the proof: *)
 (** 評価の定義を計算的なものから関係的なものに変更するのは、
     評価は全関数であるべきという (Fixpoint の定義における 
     Coq の制限によって課せられる) 不自然な要求から逃れさせてくれる良い変更です。
@@ -2181,54 +1842,32 @@ Proof.
     SCase "b1 evaluates to false".
       apply IHE1. assumption.
   Case "E_WhileEnd".
-    SCase "b1 evaluates to true".
+    SCase "b1 evaluates to false".
       reflexivity.
-    SCase "b1 evaluates to false (contradiction)".
+    SCase "b1 evaluates to true (contradiction)".
       rewrite H in H2. inversion H2.
   Case "E_WhileLoop".
-    SCase "b1 evaluates to true (contradiction)".
+    SCase "b1 evaluates to false (contradiction)".
       rewrite H in H4. inversion H4.
-    SCase "b1 evaluates to false".
+    SCase "b1 evaluates to true".
       assert (st' = st'0) as EQ1.
         SSCase "Proof of assertion". apply IHE1_1; assumption.
       subst st'0.
       apply IHE1_2. assumption.  Qed.
 
-(*  Here's a slicker proof, using the fact that the relational and
-    step-indexed definition of evaluation are the same. *)
-(** 以下に、より巧みな証明を示します。
-    これは関係による定義と指数を利用した定義の評価が同じである事実を利用しています。*)
-
-Theorem ceval_deterministic' : forall c st st1 st2,
-     c / st || st1  ->
-     c / st || st2 ->
-     st1 = st2.
-Proof.
-  intros c st st1 st2 He1 He2.
-  apply ceval__ceval_step in He1.
-  apply ceval__ceval_step in He2.
-  inversion He1 as [i1 E1].
-  inversion He2 as [i2 E2].
-  apply ceval_step_more with (i2 := i1 + i2) in E1.
-  apply ceval_step_more with (i2 := i1 + i2) in E2.
-  rewrite E1 in E2. inversion E2. reflexivity.
-  omega. omega.  Qed.
-
 (* ####################################################### *)
-(*  * Reasoning About Programs *)
-(** * プログラムの検証 *)
+(*  * Reasoning About Imp Programs *)
+(** * Imp プログラムの検証 *)
 
-(*  We'll get much deeper into systematic techniques for reasoning
-    about programs in Imp in the following chapters, but we can do
-    quite a bit just working with the bare definitions.  This section
-    explores some examples. *)
+(** We'll get much deeper into systematic techniques for reasoning
+    about Imp programs in the following chapters, but we can do quite
+    a bit just working with the bare definitions. *)
 (** ここから Imp におけるプログラムの検証に対する系統だったテクニックに深く関わっていきます。
     しかし、その多くはむき出しの (もとの) 定義を扱うだけで出来ます。
     この章では、いくつかの例を探します。*)
 
-(*  ** Basic Examples *)
-(** ** 基本的な例 *)
-
+(* This section explores some examples. *)
+(** このセクションで、いくつか例を見ていきましょう *)
 Theorem plus2_spec : forall st n st',
   st X = n ->
   plus2 / st || st' ->
@@ -2239,43 +1878,45 @@ Proof.
      step of the ceval computation - in this case revealing
      that st' must be st extended with the new value of X,
      since plus2 is an assignment *)
-  inversion Heval. subst.
+  inversion Heval. subst. clear Heval. simpl.
   apply update_eq.  Qed.
 
-(*  **** Exercise: 3 stars, recommended (XtimesYinZ_spec) *)
+(*  **** Exercise: 3 stars (XtimesYinZ_spec) *)
 (** **** 練習問題: ★★★, recommended (XtimesYinZ_spec) *)
-(*  State and prove a specification of the XtimesYinZ Imp program. *)
+(*  State and prove a specification of [XtimesYinZ]. *)
 (** XtimesYinZ の Imp プログラムの仕様を書いて証明しなさい。*)
 
 (* FILL IN HERE *)
 (** [] *)
 
-(*  **** Exercise: 3 stars, recommended (loop_never_stops) *)
-(** **** 練習問題: ★★★, recommended (loop_never_stops) *)
+(** **** Exercise: 3 stars (loop_never_stops) *)
 Theorem loop_never_stops : forall st st',
   ~(loop / st || st').
 Proof.
   intros st st' contra. unfold loop in contra.
-  remember (WHILE BTrue DO SKIP END) as loopdef.
-  (* Proceed by induction on the assumed derivation showing that
-     loopdef terminates.  Most of the cases are immediately
+  remember (WHILE BTrue DO SKIP END) as loopdef eqn:Heqloopdef.
+    (* Proceed by induction on the assumed derivation showing that
+     [loopdef] terminates.  Most of the cases are immediately
      contradictory (and so can be solved in one step with
      [inversion]). *)
   (* FILL IN HERE *) Admitted.
 (** [] *)
 
+(*  **** Exercise: 3 stars (no_whilesR) *)
+(** **** 練習問題: ★★, optional (no_whilesR) *)
+(*  Consider the definition of the [no_whiles] property below: *)
+(** 下に定義されている[no_whiles]の特徴について考えましょう *)
+
 Fixpoint no_whiles (c : com) : bool :=
   match c with
   | SKIP       => true
   | _ ::= _    => true
-  | c1 ; c2  => andb (no_whiles c1) (no_whiles c2)
+  | c1 ;; c2  => andb (no_whiles c1) (no_whiles c2)
   | IFB _ THEN ct ELSE cf FI => andb (no_whiles ct) (no_whiles cf)
   | WHILE _ DO _ END  => false
   end.
 
-(*  **** Exercise: 2 stars, optional (no_whilesR) *)
-(** **** 練習問題: ★★, optional (no_whilesR) *)
-(*  The [no_whiles] property yields [true] on just those programs that
+(*i  This property yields [true] just on programs that
     have no while loops.  Using [Inductive], write a property
     [no_whilesR] such that [no_whilesR c] is provable exactly when [c]
     is a program with no while loops.  Then prove its equivalence
@@ -2294,7 +1935,7 @@ Proof.
   (* FILL IN HERE *) Admitted.
 (** [] *)
 
-(*  **** Exercise: 4 stars, optional (no_whiles_terminating) *)
+(*  **** Exercise: 4 stars (no_whiles_terminating) *)
 (** **** 練習問題: ★★★★, optional (no_whiles_terminating) *)
 (*  Imp programs that don't involve while loops always terminate.
     State and prove a theorem that says this. *)
@@ -2306,203 +1947,11 @@ Proof.
 (* FILL IN HERE *)
 (** [] *)
 
-(*  ** Proving a Program Correct (Optional) *)
-(** ** プログラム正当性 (Optional) *)
-
-(*  Recall the factorial program: *)
-(** 階乗のプログラムを思い出しましょう: *)
-
-Print fact_body. Print fact_loop. Print fact_com.
-
-(*  Here is an alternative "mathematical" definition of the factorial
-    function: *)
-(** 階乗関数の別の「数学的な」定義を以下に示します: *)
-
-Fixpoint real_fact (n:nat) : nat :=
-  match n with
-  | O => 1
-  | S n' => n * (real_fact n')
-  end.
-
-(*  We would like to show that they agree -- if we start [fact_com] in
-    a state where variable [X] contains some number [x], then it will
-    terminate in a state where variable [Y] contains the factorial of
-    [x].
-
-    To show this, we rely on the critical idea of a _loop
-    invariant_. *)
-(** 変数 [X] がある数 [x] を持つ状態で [fact_com] を実行すると、
-    変数 [Y] が [x] の階乗の値を持つ状態で停止する、ということを示したくなります。
-    
-    これを示すため、ループ不変式 (_loop invariant_) という重要な概念を使います。 *)
-
-Definition fact_invariant (x:nat) (st:state) :=
-  (st Y) * (real_fact (st Z)) = real_fact x.
-
-Theorem fact_body_preserves_invariant: forall st st' x,
-     fact_invariant x st ->
-     st Z <> 0 ->
-     fact_body / st || st' ->
-     fact_invariant x st'.
-Proof.
-  unfold fact_invariant, fact_body.
-  intros st st' x Hm HZnz He.
-  inversion He; subst; clear He.
-  inversion H1; subst; clear H1.
-  inversion H4; subst; clear H4.
-  unfold update. simpl.
-  (* Show that st Z = S z' for some z' *)
-  destruct (st Z) as [| z'].
-    apply ex_falso_quodlibet. apply HZnz. reflexivity.
-  rewrite <- Hm. rewrite <- mult_assoc.
-  replace (S z' - 1) with z' by omega.
-  reflexivity.  Qed.
-
-Theorem fact_loop_preserves_invariant : forall st st' x,
-     fact_invariant x st ->
-     fact_loop / st || st' ->
-     fact_invariant x st'.
-Proof.
-  intros st st' x H Hce.
-  remember fact_loop as c.
-  ceval_cases (induction Hce) Case;
-              inversion Heqc; subst; clear Heqc.
-  Case "E_WhileEnd".
-    (* trivial when the loop doesn't run... *)
-    assumption.
-  Case "E_WhileLoop".
-    (* if the loop does run, we know that fact_body preserves
-       fact_invariant -- we just need to assemble the pieces *)
-    apply IHHce2.
-      apply fact_body_preserves_invariant with st;
-            try assumption.
-      intros Contra. simpl in H0; subst.
-      rewrite Contra in H0. inversion H0.
-      reflexivity.  Qed.
-
-Theorem guard_false_after_loop: forall b c st st',
-     (WHILE b DO c END) / st || st' ->
-     beval st' b = false.
-Proof.
-  intros b c st st' Hce.
-  remember (WHILE b DO c END) as cloop.
-  ceval_cases (induction Hce) Case;
-     inversion Heqcloop; subst; clear Heqcloop.
-  Case "E_WhileEnd".
-    assumption.
-  Case "E_WhileLoop".
-    apply IHHce2. reflexivity.  Qed.
-
-(*  Patching it all together... *)
-(** これらをすべてつなぎ合わせましょう... *)
-
-Theorem fact_com_correct : forall st st' x,
-     st X = x ->
-     fact_com / st || st' ->
-     st' Y = real_fact x.
-Proof.
-  intros st st' x HX Hce.
-  inversion Hce; subst; clear Hce.
-  inversion H1; subst; clear H1.
-  inversion H4; subst; clear H4.
-  inversion H1; subst; clear H1.
-  rename st' into st''. simpl in H5.
-  (* The invariant is true before the loop runs... *)
-  remember (update (update st Z (st X)) Y 1) as st'.
-  assert (fact_invariant (st X) st').
-    subst. unfold fact_invariant, update. simpl. omega.
-  (* ...so when the loop is done running, the invariant
-     is maintained *)
-  assert (fact_invariant (st X) st'').
-    apply fact_loop_preserves_invariant with st'; assumption.
-  unfold fact_invariant in H0.
-  (* Finally, if the loop terminated, then Z is 0; so Y must be
-     factorial of X *)
-  apply guard_false_after_loop in H5. simpl in H5.
-  destruct (st'' Z).
-  Case "st'' Z = 0". simpl in H0. omega.
-  Case "st'' Z > 0 (impossible)". inversion H5.
-Qed.
-
-(*  One might wonder whether all this work with poking at states and
-    unfolding definitions could be ameliorated with some more powerful
-    lemmas and/or more uniform reasoning principles... Indeed, this is
-    exactly the topic of the next chapter ([Hoare.v])! *)
-(** この、状態をつっついて定義を展開するような全体のやり方を、何かより強力な補題や、
-    より一貫性のある推論原理で改善できないのかと思う人もいるかもしれません。
-    実は、それがまさに次の章([Hoare_J.v])の主題です! *)
-
-
-(* **** Exercise: 4 stars, optional (subtract_slowly_spec) *)
-(** **** 練習問題: ★★★★, optional (subtract_slowly_spec) *)
-(** 上の [fact_com] の仕様、および以下の不変式をガイドとして、
-    subtract_slowly の仕様を証明しなさい。 *)
-
-Definition ss_invariant (x:nat) (z:nat) (st:state) :=
-  minus (st Z) (st X) = minus z x.
-
-(* FILL IN HERE *)
-(** [] *)
-
 (* ####################################################### *)
-(*  * Additional Exercises *)
-(** * 追加の練習問題 *)
+(** * Additional Exercises *)
 
-(*  **** Exercise: 4 stars, optional (add_for_loop) *)
-(** **** 練習問題: ★★★★, optional (add_for_loop) *)
-(*  Add C-style [for] loops to the language of commands, update the
-    [ceval] definition to define the semantics of [for] loops, and add
-    cases for [for] loops as needed so that all the proofs in this file
-    are accepted by Coq.
-
-    A [for] loop should be parameterized by (a) a statement executed
-    initially, (b) a test that is run on each iteration of the loop to
-    determine whether the loop should continue, (c) a statement
-    executed at the end of each loop iteration, and (d) a statement
-    that makes up the body of the loop.  (You don't need to worry
-    about making up a concrete Notation for [for] loops, but feel free
-    to play with this too if you like.) *)
-(** C 風の [for] ループをコマンドの言語に追加し、[ceval] の定義を
-   [for] ループの意味も与えるよう更新して、
-   このファイルにあるすべての証明が Coq に通るよう、
-   必要なところへ [for] ループに対する場合分けを追加しなさい。
-
-    [for] ループは (a) 初めに実行される主張、
-    (b) 各繰り返しで実行される、ループを続けてよいか決定するテスト、
-    (c) 各ループの繰り返しの最後に実行される主張、および
-    (d) ループの本体を構成する主張によってパラメタ化されていなければなりません。
-    ([for] ループに対する具体的な表記の構成を気にする必要はありませんが、
-    やりたければ自由にやって構いません。) *)
-
-(* FILL IN HERE *)
-(** [] *)
-
-(*  **** Exercise: 3 stars, optional (short_circuit) *)
-(** **** 練習問題: ★★★, optional (short_circuit) *)
-(*  Most modern programming languages use a "short-circuit" evaluation
-    rule for boolean [and]: to evaluate [BAnd b1 b2], first evaluate
-    [b1].  If it evaluates to [false], then the entire [BAnd]
-    expression evaluates to [false] immediately, without evaluating
-    [b2].  Otherwise, [b2] is evaluated to determine the result of the
-    [BAnd] expression.
-
-    Write an alternate version of [beval] that performs short-circuit
-    evaluation of [BAnd] in this manner, and prove that it is
-    equivalent to [beval]. *)
-(** 多くのモダンなプログラミング言語はブール演算子 [and] に対し、
-    「省略した」実行を使っています。
-    [BAnd b1 b2] を実行するには、まず [b1] を評価します。
-    それが [false] に評価されるならば、[b2] の評価はせず、
-    すぐに [BAnd] 式全体の結果を [false] に評価します。
-    そうでなければ、[BAnd] 式の結果を決定するため、[b2] が評価されます。
-
-    このように [BAnd] を省略して評価する、別のバージョンの [beval] を書き、
-    それが [beavl] と等価であることを証明しなさい。 *)
-
-(* FILL IN HERE *)
-
-(* **** Exercise: 4 stars, recommended (stack_compiler) *)
-(** **** 練習問題: ★★★★, recommended (stack_compiler) *)
+(*  **** Exercise: 3 stars (stack_compiler) *)
+(** **** 練習問題: ★★★, recommended (stack_compiler) *)
 (*  HP Calculators, programming languages like Forth and Postscript,
     and abstract machines like the Java Virtual Machine all evaluate
     arithmetic expressions using a stack. For instance, the expression
@@ -2528,19 +1977,17 @@ Definition ss_invariant (x:nat) (z:nat) (st:state) :=
 >>
 
   The task of this exercise is to write a small compiler that
-  translates [aexp]s into stack machine instructions, and to prove its
-  correctness.
+  translates [aexp]s into stack machine instructions.
 
   The instruction set for our stack language will consist of the
   following instructions:
      - [SPush n]: Push the number [n] on the stack.
-     - [SLoad X]: Load the identifier [X] from the store and push it
+     - [SLoad x]: Load the identifier [x] from the store and push it
                   on the stack
      - [SPlus]:   Pop the two top numbers from the stack, add them, and
                   push the result onto the stack.
      - [SMinus]:  Similar, but subtract.
-     - [SMult]:   Similar, but multiply.
-*)
+     - [SMult]:   Similar, but multiply. *)
 (** HP の電卓、Forth や Postscript などのプログラミング言語、
    および Java Virtual Machine などの抽象機械はすべて、スタックを使って算術式を評価します。
    例えば、
@@ -2574,7 +2021,6 @@ Definition ss_invariant (x:nat) (z:nat) (st:state) :=
                   結果をスタックにプッシュする。
      - [SMinus]:  上と同様。ただし引く。
      - [SMult]:   上と同様。ただし掛ける。
-*)
 
 Inductive sinstr : Type :=
 | SPush : nat -> sinstr
@@ -2583,7 +2029,7 @@ Inductive sinstr : Type :=
 | SMinus : sinstr
 | SMult : sinstr.
 
-(*  Write a function to evaluate programs in the stack language. It
+(** Write a function to evaluate programs in the stack language. It
     takes as input a state, a stack represented as a list of
     numbers (top stack item is the head of the list), and a program
     represented as a list of instructions, and returns the stack after
@@ -2591,10 +2037,9 @@ Inductive sinstr : Type :=
 
     Note that the specification leaves unspecified what to do when
     encountering an [SPlus], [SMinus], or [SMult] instruction if the
-    stack contains less than two elements.  In a sense it is
-    immaterial, since our compiler will never emit such a malformed
-    program. However, when you do the correctness proof you may find
-    some choices makes the proof easier than others. *)
+    stack contains less than two elements.  In a sense, it is
+    immaterial what we do, since our compiler will never emit such a
+    malformed program. *)
 (** スタック言語のプログラムを評価するための関数を書きなさい。
     入力として、状態、数のリストとして表現されたスタック
     (スタックの先頭要素はリストの先頭)、
@@ -2613,16 +2058,17 @@ Fixpoint s_execute (st : state) (stack : list nat)
                  : list nat :=
 (* FILL IN HERE *) admit.
 
+
 Example s_execute1 :
      s_execute empty_state []
-       [SPush 5, SPush 3, SPush 1, SMinus]
-   = [2, 5].
+       [SPush 5; SPush 3; SPush 1; SMinus]
+   = [2; 5].
 (* FILL IN HERE *) Admitted.
 
 Example s_execute2 :
-     s_execute (update empty_state X 3) [3,4]
-       [SPush 4, SLoad X, SMult, SPlus]
-   = [15, 4].
+     s_execute (update empty_state X 3) [3;4]
+       [SPush 4; SLoad X; SMult; SPlus]
+   = [15; 4].
 (* FILL IN HERE *) Admitted.
 
 (*  Next, write a function which compiles an [aexp] into a stack
@@ -2631,27 +2077,265 @@ Example s_execute2 :
 (** 次に、[aexp] をスタック機械のプログラムにコンパイルする関数を書きなさい。
     このプログラムを実行する影響は、もとの式の値をスタックに積むことと同じでなければなりません。*)
 
+
 Fixpoint s_compile (e : aexp) : list sinstr :=
 (* FILL IN HERE *) admit.
 
-(*
+(* After you've defined [s_compile], uncomment the following to test
+    that it works. *)
+(** [s_compile]の定義が終ったら、以下のコメントを外し、テストが正しく動くことを確かめなさい。*)
+(* 
 Example s_compile1 :
     s_compile (AMinus (AId X) (AMult (ANum 2) (AId Y)))
-  = [SLoad X, SPush 2, SLoad Y, SMult, SMinus].
+  = [SLoad X; SPush 2; SLoad Y; SMult; SMinus].
 Proof. reflexivity. Qed.
 *)
+(** [] *)
 
-(*  Finally, prove the following theorem, stating that the [compile]
-    function behaves correctly.  You will need to start by stating a
-    more general lemma to get a usable induction hypothesis. *)
-(** 最後に、[compile] 関数が正しく振る舞うことを述べている以下の定理を証明しなさい。
-    まずは使える帰納法の仮定を得るため、より一般的な補題を述べる必要があるでしょう。*)
+(** **** Exercise: 3 stars, advanced (stack_compiler_correct) *)
+(** The task of this exercise is to prove the correctness of the
+    calculator implemented in the previous exercise.  Remember that
+    the specification left unspecified what to do when encountering an
+    [SPlus], [SMinus], or [SMult] instruction if the stack contains
+    less than two elements.  (In order to make your correctness proof
+    easier you may find it useful to go back and change your
+    implementation!)
 
-(* FILL IN HERE *)
+    Prove the following theorem, stating that the [compile] function
+    behaves correctly.  You will need to start by stating a more
+    general lemma to get a usable induction hypothesis; the main
+    theorem will then be a simple corollary of this lemma. *)
+
 
 Theorem s_compile_correct : forall (st : state) (e : aexp),
   s_execute st [] (s_compile e) = [ aeval st e ].
 Proof.
   (* FILL IN HERE *) Admitted.
 (** [] *)
+
+(** **** Exercise: 5 stars, advanced (break_imp) *)
+Module BreakImp.
+
+(** Imperative languages such as C or Java often have a [break] or
+    similar statement for interrupting the execution of loops. In this
+    exercise we will consider how to add [break] to Imp.
+
+    First, we need to enrich the language of commands with an
+    additional case. *)
+
+Inductive com : Type :=
+  | CSkip : com
+  | CBreak : com
+  | CAss : id -> aexp -> com
+  | CSeq : com -> com -> com
+  | CIf : bexp -> com -> com -> com
+  | CWhile : bexp -> com -> com.
+
+Tactic Notation "com_cases" tactic(first) ident(c) :=
+  first;
+  [ Case_aux c "SKIP" | Case_aux c "BREAK" | Case_aux c "::=" | Case_aux c ";"
+  | Case_aux c "IFB" | Case_aux c "WHILE" ].
+
+Notation "'SKIP'" :=
+  CSkip.
+Notation "'BREAK'" :=
+  CBreak.
+Notation "x '::=' a" :=
+  (CAss x a) (at level 60).
+Notation "c1 ; c2" :=
+  (CSeq c1 c2) (at level 80, right associativity).
+Notation "'WHILE' b 'DO' c 'END'" :=
+  (CWhile b c) (at level 80, right associativity).
+Notation "'IFB' c1 'THEN' c2 'ELSE' c3 'FI'" :=
+  (CIf c1 c2 c3) (at level 80, right associativity).
+
+(** Next, we need to define the behavior of [BREAK].  Informally,
+    whenever [BREAK] is executed in a sequence of commands, it stops
+    the execution of that sequence and signals that the innermost
+    enclosing loop (if any) should terminate. If there aren't any
+    enclosing loops, then the whole program simply terminates. The
+    final state should be the same as the one in which the [BREAK]
+    statement was executed.
+
+    One important point is what to do when there are multiple loops
+    enclosing a given [BREAK]. In those cases, [BREAK] should only
+    terminate the _innermost_ loop where it occurs. Thus, after
+    executing the following piece of code...
+   X ::= 0;
+   Y ::= 1;
+   WHILE 0 <> Y DO
+     WHILE TRUE DO
+       BREAK
+     END;
+     X ::= 1;
+     Y ::= Y - 1
+   END
+    ... the value of [X] should be [1], and not [0].
+
+    One way of expressing this behavior is to add another parameter to
+    the evaluation relation that specifies whether evaluation of a
+    command executes a [BREAK] statement: *)
+
+Inductive status : Type :=
+  | SContinue : status
+  | SBreak : status.
+
+Reserved Notation "c1 '/' st '||' s '/' st'"
+                  (at level 40, st, s at level 39).
+
+(** Intuitively, [c / st || s / st'] means that, if [c] is started in
+    state [st], then it terminates in state [st'] and either signals
+    that any surrounding loop (or the whole program) should exit
+    immediately ([s = SBreak]) or that execution should continue
+    normally ([s = SContinue]).
+
+    The definition of the "[c / st || s / st']" relation is very
+    similar to the one we gave above for the regular evaluation
+    relation ([c / st || s / st']) -- we just need to handle the
+    termination signals appropriately:
+
+    - If the command is [SKIP], then the state doesn't change, and
+      execution of any enclosing loop can continue normally.
+
+    - If the command is [BREAK], the state stays unchanged, but we
+      signal a [SBreak].
+
+    - If the command is an assignment, then we update the binding for
+      that variable in the state accordingly and signal that execution
+      can continue normally.
+
+    - If the command is of the form [IF b THEN c1 ELSE c2 FI], then
+      the state is updated as in the original semantics of Imp, except
+      that we also propagate the signal from the execution of
+      whichever branch was taken.
+
+    - If the command is a sequence [c1 ; c2], we first execute
+      [c1]. If this yields a [SBreak], we skip the execution of [c2]
+      and propagate the [SBreak] signal to the surrounding context;
+      the resulting state should be the same as the one obtained by
+      executing [c1] alone. Otherwise, we execute [c2] on the state
+      obtained after executing [c1], and propagate the signal that was
+      generated there.
+
+    - Finally, for a loop of the form [WHILE b DO c END], the
+      semantics is almost the same as before. The only difference is
+      that, when [b] evaluates to true, we execute [c] and check the
+      signal that it raises. If that signal is [SContinue], then the
+      execution proceeds as in the original semantics. Otherwise, we
+      stop the execution of the loop, and the resulting state is the
+      same as the one resulting from the execution of the current
+      iteration. In either case, since [BREAK] only terminates the
+      innermost loop, [WHILE] signals [SContinue]. *)
+
+(** Based on the above description, complete the definition of the
+    [ceval] relation. *)
+
+Inductive ceval : com -> state -> status -> state -> Prop :=
+  | E_Skip : forall st,
+      CSkip / st || SContinue / st
+  (* FILL IN HERE *)
+
+  where "c1 '/' st '||' s '/' st'" := (ceval c1 st s st').
+
+Tactic Notation "ceval_cases" tactic(first) ident(c) :=
+  first;
+  [ Case_aux c "E_Skip"
+  (* FILL IN HERE *)
+  ].
+
+(** Now the following properties of your definition of [ceval]: *)
+
+Theorem break_ignore : forall c st st' s,
+     (BREAK; c) / st || s / st' ->
+     st = st'.
+Proof.
+  (* FILL IN HERE *) Admitted.
+
+Theorem while_continue : forall b c st st' s,
+  (WHILE b DO c END) / st || s / st' ->
+  s = SContinue.
+Proof.
+  (* FILL IN HERE *) Admitted.
+
+Theorem while_stops_on_break : forall b c st st',
+  beval st b = true ->
+  c / st || SBreak / st' ->
+  (WHILE b DO c END) / st || SContinue / st'.
+Proof.
+  (* FILL IN HERE *) Admitted.
+
+Theorem while_break_true : forall b c st st',
+  (WHILE b DO c END) / st || SContinue / st' ->
+  beval st' b = true ->
+  exists st'', c / st'' || SBreak / st'.
+Proof.
+(* FILL IN HERE *) Admitted.
+
+Theorem ceval_deterministic: forall (c:com) st st1 st2 s1 s2,
+     c / st || s1 / st1  ->
+     c / st || s2 / st2 ->
+     st1 = st2 /\ s1 = s2.
+Proof.
+  (* FILL IN HERE *) Admitted.
+
+End BreakImp.
+(** [] *)
+
+(*  **** Exercise: 3 stars, optional (short_circuit) *)
+(** **** 練習問題: ★★★, optional (short_circuit) *)
+(*  Most modern programming languages use a "short-circuit" evaluation
+    rule for boolean [and]: to evaluate [BAnd b1 b2], first evaluate
+    [b1].  If it evaluates to [false], then the entire [BAnd]
+    expression evaluates to [false] immediately, without evaluating
+    [b2].  Otherwise, [b2] is evaluated to determine the result of the
+    [BAnd] expression.
+
+    Write an alternate version of [beval] that performs short-circuit
+    evaluation of [BAnd] in this manner, and prove that it is
+    equivalent to [beval]. *)
+(** 多くのモダンなプログラミング言語はブール演算子 [and] に対し、
+    「省略した」実行を使っています。
+    [BAnd b1 b2] を実行するには、まず [b1] を評価します。
+    それが [false] に評価されるならば、[b2] の評価はせず、
+    すぐに [BAnd] 式全体の結果を [false] に評価します。
+    そうでなければ、[BAnd] 式の結果を決定するため、[b2] が評価されます。
+
+    このように [BAnd] を省略して評価する、別のバージョンの [beval] を書き、
+    それが [beavl] と等価であることを証明しなさい。 *)
+
+(* FILL IN HERE *)
+(** [] *)
+
+(*  **** Exercise: 4 stars, optional (add_for_loop) *)
+(** **** 練習問題: ★★★★, optional (add_for_loop) *)
+(* Add C-style [for] loops to the language of commands, update the
+    [ceval] definition to define the semantics of [for] loops, and add
+    cases for [for] loops as needed so that all the proofs in this file
+    are accepted by Coq.
+
+    A [for] loop should be parameterized by (a) a statement executed
+    initially, (b) a test that is run on each iteration of the loop to
+    determine whether the loop should continue, (c) a statement
+    executed at the end of each loop iteration, and (d) a statement
+    that makes up the body of the loop.  (You don't need to worry
+    about making up a concrete Notation for [for] loops, but feel free
+    to play with this too if you like.) *)
+(** C 風の [for] ループをコマンドの言語に追加し、[ceval] の定義を
+   [for] ループの意味も与えるよう更新して、
+   このファイルにあるすべての証明が Coq に通るよう、
+   必要なところへ [for] ループに対する場合分けを追加しなさい。
+
+    [for] ループは (a) 初めに実行される主張、
+    (b) 各繰り返しで実行される、ループを続けてよいか決定するテスト、
+    (c) 各ループの繰り返しの最後に実行される主張、および
+    (d) ループの本体を構成する主張によってパラメタ化されていなければなりません。
+    ([for] ループに対する具体的な表記の構成を気にする必要はありませんが、
+    やりたければ自由にやって構いません。) *)
+
+
+(* FILL IN HERE *)
+(** [] *)
+
+
+(* <$Date: 2013-07-17 16:19:11 -0400 (Wed, 17 Jul 2013) $ *)
 
